<?xml version="1.0"?>
<rdf:RDF xmlns="https://www.isibang.ac.in/ns/amv#"
     xml:base="https://www.isibang.ac.in/ns/amv"
     xmlns:dc="http://purl.org/dc/elements/1.1/"
     xmlns:wd="http://www.wikidata.org/entity/"
     xmlns:amv="https://www.isibang.ac.in/ns/amv#"
     xmlns:mod="http://www.isibang.ac.in/ns/mod#"
     xmlns:owl="http://www.w3.org/2002/07/owl#"
     xmlns:rdf="http://www.w3.org/1999/02/22-rdf-syntax-ns#"
     xmlns:wdt="http://www.wikidata.org/prop/direct/"
     xmlns:xml="http://www.w3.org/XML/1998/namespace"
     xmlns:xsd="http://www.w3.org/2001/XMLSchema#"
     xmlns:bibo="http://purl.org/ontology/bibo/"
     xmlns:dcat="http://www.w3.org/ns/dcat#"
     xmlns:doap="http://usefulinc.com/ns/doap/"
     xmlns:foaf="http://xmlns.com/foaf/0.1/"
     xmlns:prov="http://www.w3.org/ns/prov"
     xmlns:rdfs="http://www.w3.org/2000/01/rdf-schema#"
     xmlns:skos="http://www.w3.org/2004/02/skos/core#"
     xmlns:terms="http://purl.org/dc/terms/"
     xmlns:schema="https://schema.org/">
    <owl:Ontology rdf:about="https://www.isibang.ac.in/ns/amv">
        <owl:versionIRI rdf:resource="https://www.isibang.ac.in/ns/amv/1.0"/>
        <dc:creator xml:lang="en">Biswanath Dutta</dc:creator>
        <dc:creator xml:lang="en">Jyotima Patel</dc:creator>
        <dc:date xml:lang="en">2021-03-11T00:00:00</dc:date>
        <dc:description xml:lang="en">Metadata vocabularies are used in various domains of study. It provides an in-depth description of the resources. In this work, we develop Algorithm Metadata Vocabulary (AMV), a vocabulary for capturing and storing the metadata about the algorithms (a procedure or a set of rules that is followed step-by-step to solve a problem, especially by a computer). The snag faced by the researchers in the current time is the failure of getting relevant results when searching for algorithms in any search engine. AMV is represented as a semantic model and produced OWL file, which can be directly used by anyone interested to create and publish algorithm metadata as a knowledge graph, or to provide metadata service through SPARQL endpoint. To design the vocabulary, we propose a well-defined methodology, which considers real issues faced by the algorithm users and the practitioners. The evaluation shows a promising result.</dc:description>
        <dc:license xml:lang="en">http://creativecommons.org/publicdomain/zero/1.0/</dc:license>
        <dc:title xml:lang="en">AMV:Algorithm Metadata Vocabulary</dc:title>
        <mod:competencyQuestion xml:lang="en">CQ1: What characteristics or properties are common across all Algorithms?
CQ2: Which algorithm belongs to subject mathematics and solves combinatorial problems?
CQ3: Retrieve the list of algorithms that are implemented in python or java and have less than 7 steps?
CQ4: For a given problem, show all the available algorithms and their corresponding time complexities? 
CQ5: Retrieve all the sorting algorithms which are expressed in the form of flowchart?</mod:competencyQuestion>
        <mod:vocabularyUsed rdf:datatype="http://www.w3.org/2001/XMLSchema#anyURI">http://purl.org/dc/terms/</mod:vocabularyUsed>
        <mod:vocabularyUsed rdf:datatype="http://www.w3.org/2001/XMLSchema#anyURI">http://purl.org/ontology/bibo/</mod:vocabularyUsed>
        <mod:vocabularyUsed rdf:datatype="http://www.w3.org/2001/XMLSchema#anyURI">http://usefulinc.com/ns/doap</mod:vocabularyUsed>
        <mod:vocabularyUsed rdf:datatype="http://www.w3.org/2001/XMLSchema#anyURI">http://www.w3.org/2004/02/skos/core#</mod:vocabularyUsed>
        <mod:vocabularyUsed rdf:datatype="http://www.w3.org/2001/XMLSchema#anyURI">http://www.w3.org/ns/dcat#</mod:vocabularyUsed>
        <mod:vocabularyUsed rdf:datatype="http://www.w3.org/2001/XMLSchema#anyURI">http://www.wikidata.org/entity/</mod:vocabularyUsed>
        <mod:vocabularyUsed xml:lang="en">http://xmlns.com/foaf/0.1/</mod:vocabularyUsed>
        <mod:vocabularyUsed rdf:datatype="http://www.w3.org/2001/XMLSchema#anyURI">https://schema.org/</mod:vocabularyUsed>
        <owl:versionInfo xml:lang="en">V1.0</owl:versionInfo>
    </owl:Ontology>
    


    <!-- 
    ///////////////////////////////////////////////////////////////////////////////////////
    //
    // Annotation properties
    //
    ///////////////////////////////////////////////////////////////////////////////////////
     -->

    


    <!-- http://purl.org/dc/elements/1.1/creator -->

    <owl:AnnotationProperty rdf:about="http://purl.org/dc/elements/1.1/creator"/>
    


    <!-- http://purl.org/dc/elements/1.1/date -->

    <owl:AnnotationProperty rdf:about="http://purl.org/dc/elements/1.1/date"/>
    


    <!-- http://purl.org/dc/elements/1.1/description -->

    <owl:AnnotationProperty rdf:about="http://purl.org/dc/elements/1.1/description"/>
    


    <!-- http://purl.org/dc/elements/1.1/license -->

    <owl:AnnotationProperty rdf:about="http://purl.org/dc/elements/1.1/license"/>
    


    <!-- http://purl.org/dc/elements/1.1/title -->

    <owl:AnnotationProperty rdf:about="http://purl.org/dc/elements/1.1/title"/>
    


    <!-- http://www.isibang.ac.in/ns/mod#competencyQuestion -->

    <owl:AnnotationProperty rdf:about="http://www.isibang.ac.in/ns/mod#competencyQuestion"/>
    


    <!-- http://www.isibang.ac.in/ns/mod#vocabularyUsed -->

    <owl:AnnotationProperty rdf:about="http://www.isibang.ac.in/ns/mod#vocabularyUsed"/>
    


    <!-- http://www.w3.org/2004/02/skos/core#AltLabel -->

    <owl:AnnotationProperty rdf:about="http://www.w3.org/2004/02/skos/core#AltLabel"/>
    


    <!-- 
    ///////////////////////////////////////////////////////////////////////////////////////
    //
    // Object Properties
    //
    ///////////////////////////////////////////////////////////////////////////////////////
     -->

    


    <!-- http://purl.org/dc/terms/accessRights -->

    <owl:ObjectProperty rdf:about="http://purl.org/dc/terms/accessRights">
        <rdfs:subPropertyOf rdf:resource="http://purl.org/dc/terms/rights"/>
        <rdfs:domain>
            <owl:Class>
                <owl:unionOf rdf:parseType="Collection">
                    <rdf:Description rdf:about="https://www.isibang.ac.in/ns/amv#Algorithm"/>
                    <rdf:Description rdf:about="https://www.isibang.ac.in/ns/amv#Implementation"/>
                </owl:unionOf>
            </owl:Class>
        </rdfs:domain>
        <rdfs:range rdf:resource="http://purl.org/dc/terms/RightsStatement"/>
        <rdfs:comment xml:lang="en">Information about who access the resource or an indication of its security status. 
Access Rights may include information regarding access or restrictions based on privacy, security, or other policies. 

Examples of access rights are: Public, Internal, Department (source: https://www.dublincore.org/groups/government/accessRights/)</rdfs:comment>
        <rdfs:label xml:lang="en">access rights</rdfs:label>
    </owl:ObjectProperty>
    


    <!-- http://purl.org/dc/terms/contributor -->

    <owl:ObjectProperty rdf:about="http://purl.org/dc/terms/contributor">
        <rdfs:domain>
            <owl:Class>
                <owl:unionOf rdf:parseType="Collection">
                    <rdf:Description rdf:about="http://purl.org/ontology/bibo/Document"/>
                    <rdf:Description rdf:about="https://www.isibang.ac.in/ns/amv#Algorithm"/>
                    <rdf:Description rdf:about="https://www.isibang.ac.in/ns/amv#Implementation"/>
                </owl:unionOf>
            </owl:Class>
        </rdfs:domain>
        <rdfs:range rdf:resource="http://xmlns.com/foaf/0.1/Agent"/>
        <rdfs:comment xml:lang="en">An agent who contributes towards the algorithm.</rdfs:comment>
        <rdfs:label>contributor</rdfs:label>
    </owl:ObjectProperty>
    


    <!-- http://purl.org/dc/terms/creator -->

    <owl:ObjectProperty rdf:about="http://purl.org/dc/terms/creator">
        <rdfs:domain>
            <owl:Class>
                <owl:unionOf rdf:parseType="Collection">
                    <rdf:Description rdf:about="http://purl.org/ontology/bibo/Document"/>
                    <rdf:Description rdf:about="https://www.isibang.ac.in/ns/amv#Algorithm"/>
                    <rdf:Description rdf:about="https://www.isibang.ac.in/ns/amv#Implementation"/>
                </owl:unionOf>
            </owl:Class>
        </rdfs:domain>
        <rdfs:range rdf:resource="http://xmlns.com/foaf/0.1/Agent"/>
        <rdfs:comment xml:lang="en">The person who created the algorithm.</rdfs:comment>
        <rdfs:label>creator</rdfs:label>
    </owl:ObjectProperty>
    


    <!-- http://purl.org/dc/terms/hasPart -->

    <owl:ObjectProperty rdf:about="http://purl.org/dc/terms/hasPart">
        <owl:inverseOf rdf:resource="http://purl.org/dc/terms/isPartOf"/>
        <rdfs:domain>
            <owl:Class>
                <owl:unionOf rdf:parseType="Collection">
                    <rdf:Description rdf:about="http://purl.org/ontology/bibo/Document"/>
                    <rdf:Description rdf:about="https://www.isibang.ac.in/ns/amv#Algorithm"/>
                    <rdf:Description rdf:about="https://www.isibang.ac.in/ns/amv#Implementation"/>
                </owl:unionOf>
            </owl:Class>
        </rdfs:domain>
        <rdfs:range>
            <owl:Class>
                <owl:unionOf rdf:parseType="Collection">
                    <rdf:Description rdf:about="http://purl.org/ontology/bibo/Document"/>
                    <rdf:Description rdf:about="https://www.isibang.ac.in/ns/amv#Algorithm"/>
                    <rdf:Description rdf:about="https://www.isibang.ac.in/ns/amv#Implementation"/>
                </owl:unionOf>
            </owl:Class>
        </rdfs:range>
        <rdfs:comment>A related resource that is included either physically or logically in the described resource.(https://www.dublincore.org/specifications/dublin-core/dcmi-terms/#http://purl.org/dc/terms/isPartOf)</rdfs:comment>
        <rdfs:label>has Part</rdfs:label>
    </owl:ObjectProperty>
    


    <!-- http://purl.org/dc/terms/hasVersion -->

    <owl:ObjectProperty rdf:about="http://purl.org/dc/terms/hasVersion">
        <owl:inverseOf rdf:resource="http://purl.org/dc/terms/isVersionOf"/>
        <rdfs:domain>
            <owl:Class>
                <owl:unionOf rdf:parseType="Collection">
                    <rdf:Description rdf:about="https://www.isibang.ac.in/ns/amv#Algorithm"/>
                    <rdf:Description rdf:about="https://www.isibang.ac.in/ns/amv#Implementation"/>
                </owl:unionOf>
            </owl:Class>
        </rdfs:domain>
        <rdfs:range rdf:resource="http://purl.org/dc/elements/1.1/Version"/>
        <rdfs:comment>Version of the released Algorithm.</rdfs:comment>
        <rdfs:label>has Version</rdfs:label>
    </owl:ObjectProperty>
    


    <!-- http://purl.org/dc/terms/isPartOf -->

    <owl:ObjectProperty rdf:about="http://purl.org/dc/terms/isPartOf">
        <rdfs:domain>
            <owl:Class>
                <owl:unionOf rdf:parseType="Collection">
                    <rdf:Description rdf:about="http://purl.org/ontology/bibo/Document"/>
                    <rdf:Description rdf:about="https://www.isibang.ac.in/ns/amv#Algorithm"/>
                    <rdf:Description rdf:about="https://www.isibang.ac.in/ns/amv#Implementation"/>
                </owl:unionOf>
            </owl:Class>
        </rdfs:domain>
        <rdfs:range>
            <owl:Class>
                <owl:unionOf rdf:parseType="Collection">
                    <rdf:Description rdf:about="http://purl.org/ontology/bibo/Document"/>
                    <rdf:Description rdf:about="https://www.isibang.ac.in/ns/amv#Algorithm"/>
                    <rdf:Description rdf:about="https://www.isibang.ac.in/ns/amv#Implementation"/>
                </owl:unionOf>
            </owl:Class>
        </rdfs:range>
        <rdfs:comment>A related resource in which the described resource is physically or logically included.(https://www.dublincore.org/specifications/dublin-core/dcmi-terms/#http://purl.org/dc/terms/isPartOf)</rdfs:comment>
        <rdfs:label>is Part Of</rdfs:label>
    </owl:ObjectProperty>
    


    <!-- http://purl.org/dc/terms/isVersionOf -->

    <owl:ObjectProperty rdf:about="http://purl.org/dc/terms/isVersionOf">
        <rdfs:domain rdf:resource="http://purl.org/dc/elements/1.1/Version"/>
        <rdfs:range>
            <owl:Class>
                <owl:unionOf rdf:parseType="Collection">
                    <rdf:Description rdf:about="https://www.isibang.ac.in/ns/amv#Algorithm"/>
                    <rdf:Description rdf:about="https://www.isibang.ac.in/ns/amv#Implementation"/>
                </owl:unionOf>
            </owl:Class>
        </rdfs:range>
        <rdfs:comment>Version of the released Algorithm.</rdfs:comment>
        <rdfs:label>is Version Of</rdfs:label>
    </owl:ObjectProperty>
    


    <!-- http://purl.org/dc/terms/license -->

    <owl:ObjectProperty rdf:about="http://purl.org/dc/terms/license">
        <rdfs:domain rdf:resource="https://www.isibang.ac.in/ns/amv#Implementation"/>
        <rdfs:range rdf:resource="http://purl.org/dc/terms/LicenseDocument"/>
        <rdfs:comment xml:lang="en">The licence under which the algorithm is published.</rdfs:comment>
        <rdfs:label>license</rdfs:label>
    </owl:ObjectProperty>
    


    <!-- http://purl.org/dc/terms/rights -->

    <owl:ObjectProperty rdf:about="http://purl.org/dc/terms/rights">
        <rdfs:domain>
            <owl:Class>
                <owl:unionOf rdf:parseType="Collection">
                    <rdf:Description rdf:about="https://www.isibang.ac.in/ns/amv#Algorithm"/>
                    <rdf:Description rdf:about="https://www.isibang.ac.in/ns/amv#Implementation"/>
                </owl:unionOf>
            </owl:Class>
        </rdfs:domain>
        <rdfs:range rdf:resource="http://purl.org/dc/terms/RightsStatement"/>
        <rdfs:comment xml:lang="en">Information about rights held in and over the resource.</rdfs:comment>
        <rdfs:label xml:lang="en">rights</rdfs:label>
    </owl:ObjectProperty>
    


    <!-- http://purl.org/dc/terms/subject -->

    <owl:ObjectProperty rdf:about="http://purl.org/dc/terms/subject">
        <rdfs:subPropertyOf rdf:resource="http://www.w3.org/2002/07/owl#topObjectProperty"/>
        <rdfs:domain>
            <owl:Class>
                <owl:unionOf rdf:parseType="Collection">
                    <rdf:Description rdf:about="http://purl.org/ontology/bibo/Document"/>
                    <rdf:Description rdf:about="https://www.isibang.ac.in/ns/amv#Algorithm"/>
                    <rdf:Description rdf:about="https://www.isibang.ac.in/ns/amv#Implementation"/>
                </owl:unionOf>
            </owl:Class>
        </rdfs:domain>
        <rdfs:range rdf:resource="https://www.wikidata.org/wiki/Q11862829"/>
        <rdfs:comment xml:lang="en">The subject or the topic of an algorithm.</rdfs:comment>
        <rdfs:label>subject</rdfs:label>
    </owl:ObjectProperty>
    


    <!-- http://schema.org/comment -->

    <owl:ObjectProperty rdf:about="http://schema.org/comment">
        <rdfs:domain>
            <owl:Class>
                <owl:unionOf rdf:parseType="Collection">
                    <rdf:Description rdf:about="https://www.isibang.ac.in/ns/amv#Algorithm"/>
                    <rdf:Description rdf:about="https://www.isibang.ac.in/ns/amv#Implementation"/>
                </owl:unionOf>
            </owl:Class>
        </rdfs:domain>
        <rdfs:range rdf:resource="http://schema.org/Comment"/>
        <rdfs:comment xml:lang="en">Comments, typically from users.</rdfs:comment>
        <rdfs:label xml:lang="en">comment</rdfs:label>
    </owl:ObjectProperty>
    


    <!-- http://www.w3.org/ns/prov#wasDerivedFrom -->

    <owl:ObjectProperty rdf:about="http://www.w3.org/ns/prov#wasDerivedFrom">
        <rdfs:domain rdf:resource="https://www.isibang.ac.in/ns/amv#Algorithm"/>
        <rdfs:range rdf:resource="https://www.isibang.ac.in/ns/amv#Algorithm"/>
        <rdfs:comment>An update of an algorithm resulting in a new one, or the construction of a new algorithm based on a pre-existing algorithm.</rdfs:comment>
        <rdfs:label>was Derived From</rdfs:label>
    </owl:ObjectProperty>
    


    <!-- http://www.wikidata.org/prop/direct/p2159 -->

    <owl:ObjectProperty rdf:about="http://www.wikidata.org/prop/direct/p2159">
        <owl:inverseOf rdf:resource="https://www.isibang.ac.in/ns/amv#availableAlgorithm"/>
        <rdfs:domain rdf:resource="https://www.isibang.ac.in/ns/amv#Algorithm"/>
        <rdfs:range rdf:resource="https://www.isibang.ac.in/ns/amv#Problem"/>
        <rdfs:comment>Problem that this algorithm or method solves.(https://www.wikidata.org/wiki/Property:P2159)</rdfs:comment>
        <rdfs:comment xml:lang="en">The type of problem the algorithm solves.</rdfs:comment>
        <rdfs:label xml:lang="en">computes solution to</rdfs:label>
    </owl:ObjectProperty>
    


    <!-- http://xmlns.com/foaf/0.1/fundedBy -->

    <owl:ObjectProperty rdf:about="http://xmlns.com/foaf/0.1/fundedBy">
        <rdfs:domain>
            <owl:Class>
                <owl:unionOf rdf:parseType="Collection">
                    <rdf:Description rdf:about="https://www.isibang.ac.in/ns/amv#Algorithm"/>
                    <rdf:Description rdf:about="https://www.isibang.ac.in/ns/amv#Implementation"/>
                </owl:unionOf>
            </owl:Class>
        </rdfs:domain>
        <rdfs:range rdf:resource="http://xmlns.com/foaf/0.1/Agent"/>
        <rdfs:label>funded By</rdfs:label>
    </owl:ObjectProperty>
    


    <!-- https://schema.org/isSimilarTo -->

    <owl:ObjectProperty rdf:about="https://schema.org/isSimilarTo">
        <rdfs:domain>
            <owl:Class>
                <owl:unionOf rdf:parseType="Collection">
                    <rdf:Description rdf:about="https://www.isibang.ac.in/ns/amv#Algorithm"/>
                    <rdf:Description rdf:about="https://www.isibang.ac.in/ns/amv#Implementation"/>
                </owl:unionOf>
            </owl:Class>
        </rdfs:domain>
        <rdfs:range>
            <owl:Class>
                <owl:unionOf rdf:parseType="Collection">
                    <rdf:Description rdf:about="https://www.isibang.ac.in/ns/amv#Algorithm"/>
                    <rdf:Description rdf:about="https://www.isibang.ac.in/ns/amv#Implementation"/>
                </owl:unionOf>
            </owl:Class>
        </rdfs:range>
        <rdfs:comment xml:lang="en">A pointer to another, functionally similar product (or multiple products).</rdfs:comment>
        <rdfs:label xml:lang="en">is similar to</rdfs:label>
    </owl:ObjectProperty>
    


    <!-- https://www.isibang.ac.in/ns/amv#affliation -->

    <owl:ObjectProperty rdf:about="https://www.isibang.ac.in/ns/amv#affliation">
        <rdfs:domain rdf:resource="http://xmlns.com/foaf/0.1/Agent"/>
        <rdfs:range rdf:resource="http://xmlns.com/foaf/0.1/Agent"/>
        <rdfs:comment>An organization that the person is affiliated with. For example, a school/university.</rdfs:comment>
        <rdfs:label>affliation</rdfs:label>
    </owl:ObjectProperty>
    


    <!-- https://www.isibang.ac.in/ns/amv#algorithmAnalysisFunctionType -->

    <owl:ObjectProperty rdf:about="https://www.isibang.ac.in/ns/amv#algorithmAnalysisFunctionType">
        <rdfs:subPropertyOf rdf:resource="http://www.w3.org/2002/07/owl#topObjectProperty"/>
        <rdfs:domain rdf:resource="https://www.isibang.ac.in/ns/amv#Algorithm"/>
        <rdfs:range rdf:resource="https://www.isibang.ac.in/ns/amv#AlgorithmAnalysisFunction"/>
        <rdfs:comment xml:lang="en">The various function types for analysis of algorithms like logarithmic functions, exponential functions etc.</rdfs:comment>
        <rdfs:label xml:lang="en">algorithm analysis function type</rdfs:label>
    </owl:ObjectProperty>
    


    <!-- https://www.isibang.ac.in/ns/amv#algorithmType -->

    <owl:ObjectProperty rdf:about="https://www.isibang.ac.in/ns/amv#algorithmType">
        <rdfs:domain rdf:resource="https://www.isibang.ac.in/ns/amv#Algorithm"/>
        <rdfs:range rdf:resource="https://www.isibang.ac.in/ns/amv#AlgorithmicType"/>
        <rdfs:comment xml:lang="en">The different type of algorithmic techniques that are used to solve the various existing problems in the most optimized manner.This classification is neither exhaustive nor disjoint but highlights the various ways in which a problem can be addressed.</rdfs:comment>
        <rdfs:comment xml:lang="en">The type of algorithm.</rdfs:comment>
        <rdfs:label xml:lang="en">algorithm Type</rdfs:label>
    </owl:ObjectProperty>
    


    <!-- https://www.isibang.ac.in/ns/amv#appearedIn -->

    <owl:ObjectProperty rdf:about="https://www.isibang.ac.in/ns/amv#appearedIn">
        <rdfs:domain rdf:resource="https://www.isibang.ac.in/ns/amv#Algorithm"/>
        <rdfs:range rdf:resource="https://www.isibang.ac.in/ns/amv#InformationResource"/>
        <rdfs:comment xml:lang="en">An algorithm appeared in a publication.</rdfs:comment>
        <rdfs:label>appeared In</rdfs:label>
    </owl:ObjectProperty>
    


    <!-- https://www.isibang.ac.in/ns/amv#availableAlgorithm -->

    <owl:ObjectProperty rdf:about="https://www.isibang.ac.in/ns/amv#availableAlgorithm">
        <rdfs:comment xml:lang="en">An algorithm for a given problem.</rdfs:comment>
        <rdfs:label xml:lang="en">available algorithm</rdfs:label>
    </owl:ObjectProperty>
    


    <!-- https://www.isibang.ac.in/ns/amv#dataStructureUsed -->

    <owl:ObjectProperty rdf:about="https://www.isibang.ac.in/ns/amv#dataStructureUsed">
        <owl:inverseOf rdf:resource="https://www.isibang.ac.in/ns/amv#dataStructureUsedIn"/>
        <rdfs:domain rdf:resource="https://www.isibang.ac.in/ns/amv#Algorithm"/>
        <rdfs:range rdf:resource="https://www.isibang.ac.in/ns/amv#DataStructure"/>
        <rdfs:comment xml:lang="en">The data structure used in an algorithm.</rdfs:comment>
        <rdfs:label>data Structure Used</rdfs:label>
    </owl:ObjectProperty>
    


    <!-- https://www.isibang.ac.in/ns/amv#dataStructureUsedIn -->

    <owl:ObjectProperty rdf:about="https://www.isibang.ac.in/ns/amv#dataStructureUsedIn">
        <rdfs:domain rdf:resource="https://www.isibang.ac.in/ns/amv#DataStructure"/>
        <rdfs:range rdf:resource="https://www.isibang.ac.in/ns/amv#Algorithm"/>
        <rdfs:label>data Structure Used In</rdfs:label>
    </owl:ObjectProperty>
    


    <!-- https://www.isibang.ac.in/ns/amv#first -->

    <owl:ObjectProperty rdf:about="https://www.isibang.ac.in/ns/amv#first">
        <rdfs:subPropertyOf rdf:resource="http://www.w3.org/2002/07/owl#topObjectProperty"/>
        <owl:inverseOf rdf:resource="https://www.isibang.ac.in/ns/amv#last"/>
        <rdfs:domain rdf:resource="http://purl.org/dc/elements/1.1/Version"/>
        <rdfs:range rdf:resource="http://purl.org/dc/elements/1.1/Version"/>
        <rdfs:comment>First Version.</rdfs:comment>
        <rdfs:label>first</rdfs:label>
    </owl:ObjectProperty>
    


    <!-- https://www.isibang.ac.in/ns/amv#hasBranch -->

    <owl:ObjectProperty rdf:about="https://www.isibang.ac.in/ns/amv#hasBranch">
        <owl:inverseOf rdf:resource="https://www.isibang.ac.in/ns/amv#isBranchOf"/>
        <rdfs:domain rdf:resource="https://www.wikidata.org/wiki/Q11862829"/>
        <rdfs:range rdf:resource="https://www.wikidata.org/wiki/Q11862829"/>
        <rdfs:comment>Branch of the academic discipline.</rdfs:comment>
        <rdfs:label>has Branch</rdfs:label>
    </owl:ObjectProperty>
    


    <!-- https://www.isibang.ac.in/ns/amv#hasFormOfExpression -->

    <owl:ObjectProperty rdf:about="https://www.isibang.ac.in/ns/amv#hasFormOfExpression">
        <owl:inverseOf rdf:resource="https://www.isibang.ac.in/ns/amv#isFormOfExpression"/>
        <rdfs:domain rdf:resource="https://www.isibang.ac.in/ns/amv#Algorithm"/>
        <rdfs:range rdf:resource="https://www.isibang.ac.in/ns/amv#FormOfExpression"/>
        <rdfs:comment>The form of expression of an Algorithm.</rdfs:comment>
        <rdfs:label>has Form Of Expression</rdfs:label>
    </owl:ObjectProperty>
    


    <!-- https://www.isibang.ac.in/ns/amv#hasImplementation -->

    <owl:ObjectProperty rdf:about="https://www.isibang.ac.in/ns/amv#hasImplementation">
        <owl:inverseOf rdf:resource="https://www.isibang.ac.in/ns/amv#isImplementationOf"/>
        <rdfs:domain rdf:resource="https://www.isibang.ac.in/ns/amv#Algorithm"/>
        <rdfs:range rdf:resource="https://www.isibang.ac.in/ns/amv#Implementation"/>
        <rdfs:comment xml:lang="en">The various applications of the algorithm.</rdfs:comment>
        <rdfs:label>has Implementation</rdfs:label>
    </owl:ObjectProperty>
    


    <!-- https://www.isibang.ac.in/ns/amv#implementationInLanguage -->

    <owl:ObjectProperty rdf:about="https://www.isibang.ac.in/ns/amv#implementationInLanguage">
        <rdfs:domain rdf:resource="https://www.isibang.ac.in/ns/amv#Implementation"/>
        <rdfs:range rdf:resource="https://www.wikidata.org/wiki/Q9143#ProgrammingLanguage"/>
        <rdfs:comment xml:lang="en">In which all language the implementation of the algorithm is available.</rdfs:comment>
        <rdfs:label xml:lang="en">implementation In Language</rdfs:label>
    </owl:ObjectProperty>
    


    <!-- https://www.isibang.ac.in/ns/amv#isBranchOf -->

    <owl:ObjectProperty rdf:about="https://www.isibang.ac.in/ns/amv#isBranchOf">
        <rdf:type rdf:resource="http://www.w3.org/2002/07/owl#TransitiveProperty"/>
        <rdfs:domain rdf:resource="https://www.wikidata.org/wiki/Q11862829"/>
        <rdfs:range rdf:resource="https://www.wikidata.org/wiki/Q11862829"/>
        <rdfs:label>is Branch Of</rdfs:label>
    </owl:ObjectProperty>
    


    <!-- https://www.isibang.ac.in/ns/amv#isFormOfExpression -->

    <owl:ObjectProperty rdf:about="https://www.isibang.ac.in/ns/amv#isFormOfExpression">
        <rdfs:domain rdf:resource="https://www.isibang.ac.in/ns/amv#FormOfExpression"/>
        <rdfs:range rdf:resource="https://www.isibang.ac.in/ns/amv#Algorithm"/>
        <rdfs:comment>The form of expression of an Algorithm.</rdfs:comment>
        <rdfs:label>is Form Of Expression</rdfs:label>
    </owl:ObjectProperty>
    


    <!-- https://www.isibang.ac.in/ns/amv#isImplementationOf -->

    <owl:ObjectProperty rdf:about="https://www.isibang.ac.in/ns/amv#isImplementationOf">
        <rdfs:domain rdf:resource="https://www.isibang.ac.in/ns/amv#Implementation"/>
        <rdfs:range rdf:resource="https://www.isibang.ac.in/ns/amv#Algorithm"/>
        <rdfs:comment>The various applications of the algorithm.</rdfs:comment>
        <rdfs:label>is Implementation Of</rdfs:label>
    </owl:ObjectProperty>
    


    <!-- https://www.isibang.ac.in/ns/amv#last -->

    <owl:ObjectProperty rdf:about="https://www.isibang.ac.in/ns/amv#last">
        <rdfs:subPropertyOf rdf:resource="http://www.w3.org/2002/07/owl#topObjectProperty"/>
        <rdfs:domain rdf:resource="http://purl.org/dc/elements/1.1/Version"/>
        <rdfs:range rdf:resource="http://purl.org/dc/elements/1.1/Version"/>
        <rdfs:comment>Last Version.</rdfs:comment>
        <rdfs:label>last</rdfs:label>
    </owl:ObjectProperty>
    


    <!-- https://www.isibang.ac.in/ns/amv#loopConstruct -->

    <owl:ObjectProperty rdf:about="https://www.isibang.ac.in/ns/amv#loopConstruct">
        <rdfs:domain rdf:resource="https://www.isibang.ac.in/ns/amv#Algorithm"/>
        <rdfs:range rdf:resource="https://www.isibang.ac.in/ns/amv#LoopConstruct"/>
        <rdfs:comment xml:lang="en">The loop best suited for the algorithm.</rdfs:comment>
        <rdfs:label>loop Construct</rdfs:label>
    </owl:ObjectProperty>
    


    <!-- https://www.isibang.ac.in/ns/amv#mathematicalProperty -->

    <owl:ObjectProperty rdf:about="https://www.isibang.ac.in/ns/amv#mathematicalProperty">
        <rdfs:domain rdf:resource="https://www.isibang.ac.in/ns/amv#Algorithm"/>
        <rdfs:range rdf:resource="https://www.isibang.ac.in/ns/amv#Mathematical_Properties"/>
        <rdfs:comment xml:lang="en">The mathematical concept used to solve the problem.</rdfs:comment>
        <rdfs:label>mathematical Property</rdfs:label>
    </owl:ObjectProperty>
    


    <!-- https://www.isibang.ac.in/ns/amv#nextVersion -->

    <owl:ObjectProperty rdf:about="https://www.isibang.ac.in/ns/amv#nextVersion">
        <rdfs:subPropertyOf rdf:resource="http://www.w3.org/2002/07/owl#topObjectProperty"/>
        <owl:inverseOf rdf:resource="https://www.isibang.ac.in/ns/amv#previousVersion"/>
        <rdfs:domain rdf:resource="http://purl.org/dc/elements/1.1/Version"/>
        <rdfs:range rdf:resource="http://purl.org/dc/elements/1.1/Version"/>
        <rdfs:comment>Next Version.</rdfs:comment>
        <rdfs:label>next Version</rdfs:label>
    </owl:ObjectProperty>
    


    <!-- https://www.isibang.ac.in/ns/amv#previousVersion -->

    <owl:ObjectProperty rdf:about="https://www.isibang.ac.in/ns/amv#previousVersion">
        <rdfs:subPropertyOf rdf:resource="http://www.w3.org/2002/07/owl#topObjectProperty"/>
        <rdfs:domain rdf:resource="http://purl.org/dc/elements/1.1/Version"/>
        <rdfs:range rdf:resource="http://purl.org/dc/elements/1.1/Version"/>
        <rdfs:comment>Previous Version.</rdfs:comment>
        <rdfs:label>previous Version</rdfs:label>
    </owl:ObjectProperty>
    


    <!-- https://www.isibang.ac.in/ns/amv#runsOnOperatingSystem -->

    <owl:ObjectProperty rdf:about="https://www.isibang.ac.in/ns/amv#runsOnOperatingSystem">
        <rdfs:domain rdf:resource="https://www.isibang.ac.in/ns/amv#Implementation"/>
        <rdfs:range rdf:resource="https://schema.org/OperatingSystem"/>
        <rdfs:comment xml:lang="en">Compatible Operating System.</rdfs:comment>
        <rdfs:label xml:lang="en">runs on Operating System</rdfs:label>
    </owl:ObjectProperty>
    


    <!-- 
    ///////////////////////////////////////////////////////////////////////////////////////
    //
    // Data properties
    //
    ///////////////////////////////////////////////////////////////////////////////////////
     -->

    


    <!-- http://purl.org/dc/terms/bibliographicCitation -->

    <owl:DatatypeProperty rdf:about="http://purl.org/dc/terms/bibliographicCitation">
        <rdfs:domain>
            <owl:Class>
                <owl:unionOf rdf:parseType="Collection">
                    <rdf:Description rdf:about="https://www.isibang.ac.in/ns/amv#Algorithm"/>
                    <rdf:Description rdf:about="https://www.isibang.ac.in/ns/amv#Implementation"/>
                </owl:unionOf>
            </owl:Class>
        </rdfs:domain>
        <rdfs:range rdf:resource="http://www.w3.org/2001/XMLSchema#string"/>
        <rdfs:comment xml:lang="en">A bibliographic reference for the resource.</rdfs:comment>
        <rdfs:label xml:lang="en">bibliographic citation</rdfs:label>
    </owl:DatatypeProperty>
    


    <!-- http://purl.org/dc/terms/created -->

    <owl:DatatypeProperty rdf:about="http://purl.org/dc/terms/created">
        <rdfs:subPropertyOf rdf:resource="http://purl.org/dc/terms/date"/>
        <rdfs:domain>
            <owl:Class>
                <owl:unionOf rdf:parseType="Collection">
                    <rdf:Description rdf:about="http://purl.org/dc/elements/1.1/Version"/>
                    <rdf:Description rdf:about="http://purl.org/ontology/bibo/Document"/>
                    <rdf:Description rdf:about="https://www.isibang.ac.in/ns/amv#Algorithm"/>
                    <rdf:Description rdf:about="https://www.isibang.ac.in/ns/amv#Implementation"/>
                </owl:unionOf>
            </owl:Class>
        </rdfs:domain>
        <rdfs:range rdf:resource="http://www.w3.org/2001/XMLSchema#dateTime"/>
        <rdfs:comment xml:lang="en">The date of creation of the algorithm.</rdfs:comment>
        <rdfs:label>created</rdfs:label>
    </owl:DatatypeProperty>
    


    <!-- http://purl.org/dc/terms/date -->

    <owl:DatatypeProperty rdf:about="http://purl.org/dc/terms/date">
        <rdfs:subPropertyOf rdf:resource="http://www.w3.org/2002/07/owl#topDataProperty"/>
        <rdfs:domain>
            <owl:Class>
                <owl:unionOf rdf:parseType="Collection">
                    <rdf:Description rdf:about="http://purl.org/dc/elements/1.1/Version"/>
                    <rdf:Description rdf:about="http://purl.org/ontology/bibo/Document"/>
                    <rdf:Description rdf:about="https://www.isibang.ac.in/ns/amv#Algorithm"/>
                    <rdf:Description rdf:about="https://www.isibang.ac.in/ns/amv#Implementation"/>
                </owl:unionOf>
            </owl:Class>
        </rdfs:domain>
        <rdfs:range rdf:resource="http://www.w3.org/2001/XMLSchema#dateTime"/>
        <rdfs:comment xml:lang="en">A point or period of time associated with an event in the lifecycle of the resource.</rdfs:comment>
        <rdfs:label>date</rdfs:label>
    </owl:DatatypeProperty>
    


    <!-- http://purl.org/dc/terms/dateSubmitted -->

    <owl:DatatypeProperty rdf:about="http://purl.org/dc/terms/dateSubmitted">
        <rdfs:subPropertyOf rdf:resource="http://purl.org/dc/terms/date"/>
        <rdfs:domain>
            <owl:Class>
                <owl:unionOf rdf:parseType="Collection">
                    <rdf:Description rdf:about="http://purl.org/dc/elements/1.1/Version"/>
                    <rdf:Description rdf:about="http://purl.org/ontology/bibo/Document"/>
                    <rdf:Description rdf:about="https://www.isibang.ac.in/ns/amv#Algorithm"/>
                    <rdf:Description rdf:about="https://www.isibang.ac.in/ns/amv#Implementation"/>
                </owl:unionOf>
            </owl:Class>
        </rdfs:domain>
        <rdfs:range rdf:resource="http://www.w3.org/2001/XMLSchema#dateTime"/>
        <rdfs:comment xml:lang="en">Date of submission of the resource.</rdfs:comment>
        <rdfs:label>dateSubmitted</rdfs:label>
    </owl:DatatypeProperty>
    


    <!-- http://purl.org/dc/terms/description -->

    <owl:DatatypeProperty rdf:about="http://purl.org/dc/terms/description">
        <rdfs:domain rdf:resource="http://www.w3.org/2002/07/owl#Thing"/>
        <rdfs:range rdf:resource="http://www.w3.org/2001/XMLSchema#string"/>
        <rdfs:comment xml:lang="en">A statement that represents something in words. It is the act of describing something. The description can include, for instance, the purpose of a thing, the scope, the area of applications of a thing, the history, etc.</rdfs:comment>
        <rdfs:label>description</rdfs:label>
    </owl:DatatypeProperty>
    


    <!-- http://purl.org/dc/terms/identifier -->

    <owl:DatatypeProperty rdf:about="http://purl.org/dc/terms/identifier">
        <rdfs:domain>
            <owl:Class>
                <owl:unionOf rdf:parseType="Collection">
                    <rdf:Description rdf:about="https://www.isibang.ac.in/ns/amv#Algorithm"/>
                    <rdf:Description rdf:about="https://www.isibang.ac.in/ns/amv#Implementation"/>
                </owl:unionOf>
            </owl:Class>
        </rdfs:domain>
        <rdfs:range rdf:resource="http://www.w3.org/2001/XMLSchema#anyURI"/>
        <rdfs:comment xml:lang="en">The unique address to the location of an algorithm and/or an implementation.</rdfs:comment>
        <rdfs:label>identifier</rdfs:label>
    </owl:DatatypeProperty>
    


    <!-- http://purl.org/dc/terms/modified -->

    <owl:DatatypeProperty rdf:about="http://purl.org/dc/terms/modified">
        <rdfs:subPropertyOf rdf:resource="http://purl.org/dc/terms/date"/>
        <rdfs:domain>
            <owl:Class>
                <owl:unionOf rdf:parseType="Collection">
                    <rdf:Description rdf:about="http://purl.org/dc/elements/1.1/Version"/>
                    <rdf:Description rdf:about="http://purl.org/ontology/bibo/Document"/>
                    <rdf:Description rdf:about="https://www.isibang.ac.in/ns/amv#Algorithm"/>
                    <rdf:Description rdf:about="https://www.isibang.ac.in/ns/amv#Implementation"/>
                </owl:unionOf>
            </owl:Class>
        </rdfs:domain>
        <rdfs:range rdf:resource="http://www.w3.org/2001/XMLSchema#dateTime"/>
        <rdfs:comment xml:lang="en">Date on which the resource was changed.</rdfs:comment>
        <rdfs:label>modified</rdfs:label>
    </owl:DatatypeProperty>
    


    <!-- http://purl.org/dc/terms/title -->

    <owl:DatatypeProperty rdf:about="http://purl.org/dc/terms/title">
        <rdfs:domain rdf:resource="http://www.w3.org/2002/07/owl#Thing"/>
        <rdfs:range rdf:resource="http://www.w3.org/2001/XMLSchema#string"/>
        <rdfs:comment xml:lang="en">A name given to the resource (e.g., book, algorithm, research software).</rdfs:comment>
        <rdfs:label>title</rdfs:label>
    </owl:DatatypeProperty>
    


    <!-- http://www.w3.org/ns/dcat#byteSize -->

    <owl:DatatypeProperty rdf:about="http://www.w3.org/ns/dcat#byteSize">
        <rdfs:domain rdf:resource="https://www.isibang.ac.in/ns/amv#Implementation"/>
        <rdfs:range rdf:resource="http://www.w3.org/2001/XMLSchema#decimal"/>
        <rdfs:comment xml:lang="en">The size of a distribution in bytes.</rdfs:comment>
        <rdfs:label xml:lang="en">byte size</rdfs:label>
    </owl:DatatypeProperty>
    


    <!-- http://www.w3.org/ns/dcat#landingPage -->

    <owl:DatatypeProperty rdf:about="http://www.w3.org/ns/dcat#landingPage">
        <rdfs:subPropertyOf rdf:resource="http://xmlns.com/foaf/0.1/page"/>
        <rdfs:range rdf:resource="http://www.w3.org/2001/XMLSchema#anyURI"/>
        <rdfs:comment xml:lang="en">A Web page that can be navigated to in a Web browser to gain access to the catalog, a dataset, its distributions and/or additional information.</rdfs:comment>
        <rdfs:label>landingPage</rdfs:label>
    </owl:DatatypeProperty>
    


    <!-- http://www.wikidata.org/prop/direct/P1249 -->

    <owl:DatatypeProperty rdf:about="http://www.wikidata.org/prop/direct/P1249">
        <rdfs:domain rdf:resource="https://www.isibang.ac.in/ns/amv#Algorithm"/>
        <rdfs:range rdf:resource="http://www.w3.org/2001/XMLSchema#dateTime"/>
        <rdfs:comment>First time a subject was mentioned in writing.(https://www.wikidata.org/wiki/Property:P1249)</rdfs:comment>
        <rdfs:label xml:lang="en">time of earliest written record</rdfs:label>
    </owl:DatatypeProperty>
    


    <!-- http://www.wikidata.org/prop/direct/P3752 -->

    <owl:DatatypeProperty rdf:about="http://www.wikidata.org/prop/direct/P3752">
        <rdfs:subPropertyOf rdf:resource="https://www.isibang.ac.in/ns/amv#timeComplexity"/>
        <rdfs:range rdf:resource="http://www.w3.org/2001/XMLSchema#string"/>
        <rdfs:comment xml:lang="en">Time complexity of an algorithm at most. (https://www.wikidata.org/wiki/Property:P3752)</rdfs:comment>
        <rdfs:label xml:lang="en">worst case time complexity</rdfs:label>
    </owl:DatatypeProperty>
    


    <!-- http://www.wikidata.org/prop/direct/P3753 -->

    <owl:DatatypeProperty rdf:about="http://www.wikidata.org/prop/direct/P3753">
        <rdfs:subPropertyOf rdf:resource="https://www.isibang.ac.in/ns/amv#timeComplexity"/>
        <rdfs:range rdf:resource="http://www.w3.org/2001/XMLSchema#string"/>
        <rdfs:comment xml:lang="en">Time complexity of an algorithm at least. (https://www.wikidata.org/wiki/Property:P3753)</rdfs:comment>
        <rdfs:label xml:lang="en">best case time complexity</rdfs:label>
    </owl:DatatypeProperty>
    


    <!-- http://www.wikidata.org/prop/direct/P3754 -->

    <owl:DatatypeProperty rdf:about="http://www.wikidata.org/prop/direct/P3754">
        <rdfs:subPropertyOf rdf:resource="https://www.isibang.ac.in/ns/amv#timeComplexity"/>
        <rdfs:range rdf:resource="http://www.w3.org/2001/XMLSchema#string"/>
        <rdfs:comment xml:lang="en">Time complexity of an algorithm on average. (https://www.wikidata.org/wiki/Property:P3754)</rdfs:comment>
        <rdfs:label xml:lang="en">average case time complexity</rdfs:label>
    </owl:DatatypeProperty>
    


    <!-- http://www.wikidata.org/prop/direct/P3755 -->

    <owl:DatatypeProperty rdf:about="http://www.wikidata.org/prop/direct/P3755">
        <rdfs:subPropertyOf rdf:resource="https://www.isibang.ac.in/ns/amv#spaceComplexity"/>
        <rdfs:range rdf:resource="http://www.w3.org/2001/XMLSchema#string"/>
        <rdfs:comment>Space complexity of an algorithm at most.(https://www.wikidata.org/wiki/Property:P3755)</rdfs:comment>
        <rdfs:label xml:lang="en">worst case space complexity</rdfs:label>
    </owl:DatatypeProperty>
    


    <!-- http://www.wikidata.org/prop/direct/P3756 -->

    <owl:DatatypeProperty rdf:about="http://www.wikidata.org/prop/direct/P3756">
        <rdfs:subPropertyOf rdf:resource="https://www.isibang.ac.in/ns/amv#spaceComplexity"/>
        <rdfs:range rdf:resource="http://www.w3.org/2001/XMLSchema#string"/>
        <rdfs:comment>Space complexity of an algorithm at least.(https://www.wikidata.org/wiki/Property:P3756)</rdfs:comment>
        <rdfs:label xml:lang="en">best case space complexity</rdfs:label>
    </owl:DatatypeProperty>
    


    <!-- http://www.wikidata.org/prop/direct/P3757 -->

    <owl:DatatypeProperty rdf:about="http://www.wikidata.org/prop/direct/P3757">
        <rdfs:subPropertyOf rdf:resource="https://www.isibang.ac.in/ns/amv#spaceComplexity"/>
        <rdfs:range rdf:resource="http://www.w3.org/2001/XMLSchema#string"/>
        <rdfs:comment>Space complexity of an algorithm on average.(https://www.wikidata.org/wiki/Property:P3757)</rdfs:comment>
        <rdfs:label xml:lang="en">average case space complexity</rdfs:label>
    </owl:DatatypeProperty>
    


    <!-- http://www.wikidata.org/prop/direct/p2534 -->

    <owl:DatatypeProperty rdf:about="http://www.wikidata.org/prop/direct/p2534">
        <rdfs:domain rdf:resource="https://www.isibang.ac.in/ns/amv#Mathematical_Properties"/>
        <rdfs:range rdf:resource="http://www.w3.org/2001/XMLSchema#string"/>
        <rdfs:comment xml:lang="en">The mathematical formula used for solving the problem.	
Mathematical formula representing a theorem or law.</rdfs:comment>
        <rdfs:label xml:lang="en">defining formula</rdfs:label>
    </owl:DatatypeProperty>
    


    <!-- http://www.wikidata.org/prop/direct/p4945 -->

    <owl:DatatypeProperty rdf:about="http://www.wikidata.org/prop/direct/p4945">
        <rdfs:domain>
            <owl:Class>
                <owl:unionOf rdf:parseType="Collection">
                    <rdf:Description rdf:about="https://www.isibang.ac.in/ns/amv#Algorithm"/>
                    <rdf:Description rdf:about="https://www.isibang.ac.in/ns/amv#Implementation"/>
                </owl:unionOf>
            </owl:Class>
        </rdfs:domain>
        <rdfs:range rdf:resource="http://www.w3.org/2001/XMLSchema#anyURI"/>
        <rdfs:comment xml:lang="en">URL which can be used to download a work.</rdfs:comment>
        <rdfs:label xml:lang="en">download link</rdfs:label>
    </owl:DatatypeProperty>
    


    <!-- http://xmlns.com/foaf/0.1/depiction -->

    <owl:DatatypeProperty rdf:about="http://xmlns.com/foaf/0.1/depiction">
        <rdfs:domain rdf:resource="http://www.w3.org/2002/07/owl#Thing"/>
        <rdfs:range rdf:resource="http://www.w3.org/2001/XMLSchema#anyURI"/>
        <rdfs:comment xml:lang="en">A depiction of some thing.</rdfs:comment>
        <rdfs:label>depiction</rdfs:label>
    </owl:DatatypeProperty>
    


    <!-- http://xmlns.com/foaf/0.1/firstName -->

    <owl:DatatypeProperty rdf:about="http://xmlns.com/foaf/0.1/firstName">
        <rdfs:domain rdf:resource="http://xmlns.com/foaf/0.1/Person"/>
        <rdfs:range rdf:resource="http://www.w3.org/2001/XMLSchema#string"/>
        <rdfs:comment xml:lang="en">The first name of a person.</rdfs:comment>
        <rdfs:label>firstName</rdfs:label>
    </owl:DatatypeProperty>
    


    <!-- http://xmlns.com/foaf/0.1/homepage -->

    <owl:DatatypeProperty rdf:about="http://xmlns.com/foaf/0.1/homepage">
        <rdfs:domain rdf:resource="http://www.w3.org/2002/07/owl#Thing"/>
        <rdfs:range rdf:resource="http://www.w3.org/2001/XMLSchema#anyURI"/>
        <rdfs:comment xml:lang="en">A homepage for some thing.</rdfs:comment>
        <rdfs:label>homepage</rdfs:label>
    </owl:DatatypeProperty>
    


    <!-- http://xmlns.com/foaf/0.1/lastName -->

    <owl:DatatypeProperty rdf:about="http://xmlns.com/foaf/0.1/lastName">
        <rdfs:domain rdf:resource="http://xmlns.com/foaf/0.1/Person"/>
        <rdfs:range rdf:resource="http://www.w3.org/2001/XMLSchema#string"/>
        <rdfs:comment xml:lang="en">The last name of a person.</rdfs:comment>
        <rdfs:label>lastName</rdfs:label>
    </owl:DatatypeProperty>
    


    <!-- http://xmlns.com/foaf/0.1/mbox -->

    <owl:DatatypeProperty rdf:about="http://xmlns.com/foaf/0.1/mbox">
        <rdfs:domain rdf:resource="http://xmlns.com/foaf/0.1/Agent"/>
        <rdfs:range rdf:resource="http://www.w3.org/2001/XMLSchema#string"/>
        <rdfs:comment xml:lang="en">A personal mailbox, ie. an Internet mailbox associated with exactly one owner, the first owner of this mailbox. This is a &apos;static inverse functional property&apos;, in that there is (across time and change) at most one individual that ever has any particular value for foaf:mbox.</rdfs:comment>
        <rdfs:label xml:lang="en">personal mailbox</rdfs:label>
    </owl:DatatypeProperty>
    


    <!-- http://xmlns.com/foaf/0.1/name -->

    <owl:DatatypeProperty rdf:about="http://xmlns.com/foaf/0.1/name">
        <rdfs:domain rdf:resource="http://www.w3.org/2002/07/owl#Thing"/>
        <rdfs:range rdf:resource="http://www.w3.org/2001/XMLSchema#string"/>
        <rdfs:comment xml:lang="en">The name for some thing.</rdfs:comment>
        <rdfs:label>name</rdfs:label>
    </owl:DatatypeProperty>
    


    <!-- http://xmlns.com/foaf/0.1/page -->

    <owl:DatatypeProperty rdf:about="http://xmlns.com/foaf/0.1/page">
        <rdfs:domain rdf:resource="http://www.w3.org/2002/07/owl#Thing"/>
        <rdfs:range rdf:resource="http://www.w3.org/2001/XMLSchema#anyURI"/>
        <rdfs:comment xml:lang="en">A page or document about this thing.</rdfs:comment>
        <rdfs:label>page</rdfs:label>
    </owl:DatatypeProperty>
    


    <!-- https://www.isibang.ac.in/ns/amv#Accessibility -->

    <owl:DatatypeProperty rdf:about="https://www.isibang.ac.in/ns/amv#Accessibility">
        <rdfs:domain rdf:resource="https://www.isibang.ac.in/ns/amv#Algorithm"/>
        <rdfs:range rdf:resource="http://www.w3.org/2001/XMLSchema#string"/>
        <rdfs:comment xml:lang="en">The information on access(i.e modify, read, download) to the algorithm.</rdfs:comment>
        <rdfs:label xml:lang="en">accessibility</rdfs:label>
    </owl:DatatypeProperty>
    


    <!-- https://www.isibang.ac.in/ns/amv#Accuracy -->

    <owl:DatatypeProperty rdf:about="https://www.isibang.ac.in/ns/amv#Accuracy">
        <rdfs:domain rdf:resource="https://www.isibang.ac.in/ns/amv#Algorithm"/>
        <rdfs:range rdf:resource="http://www.w3.org/2001/XMLSchema#decimal"/>
        <rdfs:comment xml:lang="en">How close the output will be to a set point.</rdfs:comment>
        <rdfs:label>accuracy</rdfs:label>
    </owl:DatatypeProperty>
    


    <!-- https://www.isibang.ac.in/ns/amv#CPU_Time_Limit -->

    <owl:DatatypeProperty rdf:about="https://www.isibang.ac.in/ns/amv#CPU_Time_Limit">
        <rdfs:domain rdf:resource="https://www.isibang.ac.in/ns/amv#Implementation"/>
        <rdfs:range rdf:resource="http://www.w3.org/2001/XMLSchema#integer"/>
        <rdfs:comment xml:lang="en">Time taken by CPU while executing the program.(In seconds)</rdfs:comment>
        <rdfs:label xml:lang="en">cpu time limit</rdfs:label>
    </owl:DatatypeProperty>
    


    <!-- https://www.isibang.ac.in/ns/amv#Constraint -->

    <owl:DatatypeProperty rdf:about="https://www.isibang.ac.in/ns/amv#Constraint">
        <rdfs:domain rdf:resource="https://www.isibang.ac.in/ns/amv#Algorithm"/>
        <rdfs:range rdf:resource="http://www.w3.org/2001/XMLSchema#string"/>
        <rdfs:comment xml:lang="en">Limitations that an algorithm posses.</rdfs:comment>
        <rdfs:label xml:lang="en">constraint</rdfs:label>
    </owl:DatatypeProperty>
    


    <!-- https://www.isibang.ac.in/ns/amv#OfflineAlgorithm -->

    <owl:DatatypeProperty rdf:about="https://www.isibang.ac.in/ns/amv#OfflineAlgorithm">
        <rdfs:domain rdf:resource="https://www.isibang.ac.in/ns/amv#Algorithm"/>
        <rdfs:range rdf:resource="http://www.w3.org/2001/XMLSchema#boolean"/>
        <rdfs:comment xml:lang="en">The complete dataset is required to start processing.</rdfs:comment>
        <rdfs:label xml:lang="en">offline algorithm</rdfs:label>
    </owl:DatatypeProperty>
    


    <!-- https://www.isibang.ac.in/ns/amv#Optimal -->

    <owl:DatatypeProperty rdf:about="https://www.isibang.ac.in/ns/amv#Optimal">
        <rdfs:domain rdf:resource="https://www.isibang.ac.in/ns/amv#Algorithm"/>
        <rdfs:range rdf:resource="http://www.w3.org/2001/XMLSchema#boolean"/>
        <rdfs:comment xml:lang="en">An algorithm is optimal means the time complexity in the worst case is is a lower bound of the function that describes the time complexity in the worst case of a problem that the algorithm in question solves.</rdfs:comment>
        <rdfs:label xml:lang="en">optimal</rdfs:label>
    </owl:DatatypeProperty>
    


    <!-- https://www.isibang.ac.in/ns/amv#Rating -->

    <owl:DatatypeProperty rdf:about="https://www.isibang.ac.in/ns/amv#Rating">
        <rdfs:domain rdf:resource="https://www.isibang.ac.in/ns/amv#Algorithm"/>
        <rdfs:range rdf:resource="http://www.w3.org/2001/XMLSchema#integer"/>
        <rdfs:comment xml:lang="en">Rating given on the basis of usefulness for the corresponding problem.</rdfs:comment>
        <rdfs:label xml:lang="en">rating</rdfs:label>
    </owl:DatatypeProperty>
    


    <!-- https://www.isibang.ac.in/ns/amv#Readable -->

    <owl:DatatypeProperty rdf:about="https://www.isibang.ac.in/ns/amv#Readable">
        <rdfs:domain rdf:resource="https://www.isibang.ac.in/ns/amv#Algorithm"/>
        <rdfs:range rdf:resource="http://www.w3.org/2001/XMLSchema#boolean"/>
        <rdfs:comment xml:lang="en">Is the algorithm readable/understandable to the user.</rdfs:comment>
        <rdfs:label xml:lang="en">readable</rdfs:label>
    </owl:DatatypeProperty>
    


    <!-- https://www.isibang.ac.in/ns/amv#edgeCase -->

    <owl:DatatypeProperty rdf:about="https://www.isibang.ac.in/ns/amv#edgeCase">
        <rdfs:domain rdf:resource="https://www.isibang.ac.in/ns/amv#Algorithm"/>
        <rdfs:range rdf:resource="http://www.w3.org/2001/XMLSchema#string"/>
        <rdfs:comment xml:lang="en">Input values that require special handling in an algorithm. When using the algorithm at an extreme(maximum or minimum) operating parameters.</rdfs:comment>
        <rdfs:label xml:lang="en">edge Case</rdfs:label>
    </owl:DatatypeProperty>
    


    <!-- https://www.isibang.ac.in/ns/amv#flexible -->

    <owl:DatatypeProperty rdf:about="https://www.isibang.ac.in/ns/amv#flexible">
        <rdfs:domain rdf:resource="https://www.isibang.ac.in/ns/amv#Algorithm"/>
        <rdfs:range rdf:resource="http://www.w3.org/2001/XMLSchema#boolean"/>
        <rdfs:comment xml:lang="en">The algorithm written in such a way that it allows to add new features without changing the existing module.</rdfs:comment>
        <rdfs:label>flexible</rdfs:label>
    </owl:DatatypeProperty>
    


    <!-- https://www.isibang.ac.in/ns/amv#input -->

    <owl:DatatypeProperty rdf:about="https://www.isibang.ac.in/ns/amv#input">
        <rdfs:domain>
            <owl:Class>
                <owl:unionOf rdf:parseType="Collection">
                    <rdf:Description rdf:about="https://www.isibang.ac.in/ns/amv#Algorithm"/>
                    <rdf:Description rdf:about="https://www.isibang.ac.in/ns/amv#Implementation"/>
                </owl:unionOf>
            </owl:Class>
        </rdfs:domain>
        <rdfs:range rdf:resource="http://www.w3.org/2001/XMLSchema#string"/>
        <rdfs:comment xml:lang="en">Something that is operated on by any process or system. An algorithm can have zero or more inputs.</rdfs:comment>
        <rdfs:label xml:lang="en">input</rdfs:label>
    </owl:DatatypeProperty>
    


    <!-- https://www.isibang.ac.in/ns/amv#libraryURI -->

    <owl:DatatypeProperty rdf:about="https://www.isibang.ac.in/ns/amv#libraryURI">
        <rdfs:domain>
            <owl:Class>
                <owl:unionOf rdf:parseType="Collection">
                    <rdf:Description rdf:about="https://www.isibang.ac.in/ns/amv#Algorithm"/>
                    <rdf:Description rdf:about="https://www.isibang.ac.in/ns/amv#Implementation"/>
                </owl:unionOf>
            </owl:Class>
        </rdfs:domain>
        <rdfs:range rdf:resource="http://www.w3.org/2001/XMLSchema#anyURI"/>
        <rdfs:comment xml:lang="en">Unique identifier of the central place where the algorithm is stored.</rdfs:comment>
        <rdfs:label>library URI</rdfs:label>
    </owl:DatatypeProperty>
    


    <!-- https://www.isibang.ac.in/ns/amv#numberOfNestedLoops -->

    <owl:DatatypeProperty rdf:about="https://www.isibang.ac.in/ns/amv#numberOfNestedLoops">
        <rdfs:domain rdf:resource="https://www.isibang.ac.in/ns/amv#Algorithm"/>
        <rdfs:range rdf:resource="http://www.w3.org/2001/XMLSchema#nonNegativeInteger"/>
        <rdfs:comment xml:lang="en">The number of nested loops in an algorithm.</rdfs:comment>
        <rdfs:label>number Of Nested Loops</rdfs:label>
    </owl:DatatypeProperty>
    


    <!-- https://www.isibang.ac.in/ns/amv#numberOfSteps -->

    <owl:DatatypeProperty rdf:about="https://www.isibang.ac.in/ns/amv#numberOfSteps">
        <rdfs:domain rdf:resource="https://www.isibang.ac.in/ns/amv#Algorithm"/>
        <rdfs:range rdf:resource="http://www.w3.org/2001/XMLSchema#nonNegativeInteger"/>
        <rdfs:comment xml:lang="en">Total number of steps that the algorithm takes to solve a certain problem.</rdfs:comment>
        <rdfs:label>number Of Steps</rdfs:label>
    </owl:DatatypeProperty>
    


    <!-- https://www.isibang.ac.in/ns/amv#onlineAlgorithm -->

    <owl:DatatypeProperty rdf:about="https://www.isibang.ac.in/ns/amv#onlineAlgorithm">
        <rdfs:domain rdf:resource="https://www.isibang.ac.in/ns/amv#Algorithm"/>
        <rdfs:range rdf:resource="http://www.w3.org/2001/XMLSchema#boolean"/>
        <rdfs:comment xml:lang="en">The data can be feed while processing.</rdfs:comment>
        <rdfs:label xml:lang="en">online algorithm</rdfs:label>
    </owl:DatatypeProperty>
    


    <!-- https://www.isibang.ac.in/ns/amv#output -->

    <owl:DatatypeProperty rdf:about="https://www.isibang.ac.in/ns/amv#output">
        <rdfs:domain>
            <owl:Class>
                <owl:unionOf rdf:parseType="Collection">
                    <rdf:Description rdf:about="https://www.isibang.ac.in/ns/amv#Algorithm"/>
                    <rdf:Description rdf:about="https://www.isibang.ac.in/ns/amv#Implementation"/>
                </owl:unionOf>
            </owl:Class>
        </rdfs:domain>
        <rdfs:range rdf:resource="http://www.w3.org/2001/XMLSchema#string"/>
        <rdfs:comment>Output after processing the input.</rdfs:comment>
        <rdfs:label xml:lang="en">output</rdfs:label>
    </owl:DatatypeProperty>
    


    <!-- https://www.isibang.ac.in/ns/amv#precision -->

    <owl:DatatypeProperty rdf:about="https://www.isibang.ac.in/ns/amv#precision">
        <rdfs:domain rdf:resource="https://www.isibang.ac.in/ns/amv#Algorithm"/>
        <rdfs:range rdf:resource="http://www.w3.org/2001/XMLSchema#float"/>
        <rdfs:comment xml:lang="en">It is a measure of quality, higher precision means algorithm returns more relevant results than irrelevant ones.</rdfs:comment>
    </owl:DatatypeProperty>
    


    <!-- https://www.isibang.ac.in/ns/amv#readme -->

    <owl:DatatypeProperty rdf:about="https://www.isibang.ac.in/ns/amv#readme">
        <rdfs:domain rdf:resource="https://www.isibang.ac.in/ns/amv#Algorithm"/>
        <rdfs:range rdf:resource="http://www.w3.org/2001/XMLSchema#string"/>
        <rdfs:comment xml:lang="en">Provide a description or Link to algorithm Readme file.</rdfs:comment>
        <rdfs:label xml:lang="en">read me</rdfs:label>
    </owl:DatatypeProperty>
    


    <!-- https://www.isibang.ac.in/ns/amv#recall -->

    <owl:DatatypeProperty rdf:about="https://www.isibang.ac.in/ns/amv#recall">
        <rdfs:domain rdf:resource="https://www.isibang.ac.in/ns/amv#Algorithm"/>
        <rdfs:range rdf:resource="http://www.w3.org/2001/XMLSchema#float"/>
        <rdfs:comment xml:lang="en">percentage of total relevent result correctly classified by the algorithm.</rdfs:comment>
        <rdfs:label xml:lang="en">recall</rdfs:label>
    </owl:DatatypeProperty>
    


    <!-- https://www.isibang.ac.in/ns/amv#spaceComplexity -->

    <owl:DatatypeProperty rdf:about="https://www.isibang.ac.in/ns/amv#spaceComplexity">
        <rdfs:domain rdf:resource="https://www.isibang.ac.in/ns/amv#Algorithm"/>
        <rdfs:range rdf:resource="http://www.w3.org/2001/XMLSchema#string"/>
        <rdfs:comment xml:lang="en">Space complexity of an algorithm quantifies the amount of space or memory taken by an algorithm to run as a function of the length of the input.</rdfs:comment>
        <rdfs:comment xml:lang="en">space complexity</rdfs:comment>
    </owl:DatatypeProperty>
    


    <!-- https://www.isibang.ac.in/ns/amv#timeComplexity -->

    <owl:DatatypeProperty rdf:about="https://www.isibang.ac.in/ns/amv#timeComplexity">
        <rdfs:domain rdf:resource="https://www.isibang.ac.in/ns/amv#Algorithm"/>
        <rdfs:range rdf:resource="http://www.w3.org/2001/XMLSchema#string"/>
        <rdfs:comment xml:lang="en">Time complexity of an algorithm quantifies the amount of time taken by an algorithm to run as a function of the length of the input.</rdfs:comment>
        <rdfs:label xml:lang="en">time complexity</rdfs:label>
    </owl:DatatypeProperty>
    


    <!-- 
    ///////////////////////////////////////////////////////////////////////////////////////
    //
    // Classes
    //
    ///////////////////////////////////////////////////////////////////////////////////////
     -->

    


    <!-- http://purl.org/dc/elements/1.1/Version -->

    <owl:Class rdf:about="http://purl.org/dc/elements/1.1/Version">
        <rdfs:comment>Version of the released Algorithm.</rdfs:comment>
        <rdfs:label>Version</rdfs:label>
    </owl:Class>
    


    <!-- http://purl.org/dc/terms/LicenseDocument -->

    <owl:Class rdf:about="http://purl.org/dc/terms/LicenseDocument">
        <rdfs:subClassOf rdf:resource="http://purl.org/dc/terms/RightsStatement"/>
        <rdfs:comment xml:lang="en">A legal document giving official permission to do something with a Resource.</rdfs:comment>
        <rdfs:label>LicenseDocument</rdfs:label>
    </owl:Class>
    


    <!-- http://purl.org/dc/terms/RightsStatement -->

    <owl:Class rdf:about="http://purl.org/dc/terms/RightsStatement">
        <rdfs:comment xml:lang="en">A statement about the intellectual property rights (IPR) held in or over a Resource, a legal document giving official permission to do something with a resource, or a statement about access rights.</rdfs:comment>
        <rdfs:label>Rights Statement</rdfs:label>
    </owl:Class>
    


    <!-- http://purl.org/ontology/bibo/AcademicArticle -->

    <owl:Class rdf:about="http://purl.org/ontology/bibo/AcademicArticle">
        <rdfs:subClassOf rdf:resource="http://purl.org/ontology/bibo/Article"/>
        <rdfs:comment xml:lang="en">A scholarly academic article, typically published in a journal.</rdfs:comment>
        <rdfs:label xml:lang="en">Academic article</rdfs:label>
    </owl:Class>
    


    <!-- http://purl.org/ontology/bibo/Article -->

    <owl:Class rdf:about="http://purl.org/ontology/bibo/Article">
        <rdfs:subClassOf rdf:resource="http://purl.org/ontology/bibo/Document"/>
        <rdfs:comment xml:lang="en">A written composition in prose, usually nonfiction, on a specific topic, forming an independent part of a book or other publication, as a newspaper or magazine.</rdfs:comment>
        <rdfs:label xml:lang="en">Article</rdfs:label>
    </owl:Class>
    


    <!-- http://purl.org/ontology/bibo/Book -->

    <owl:Class rdf:about="http://purl.org/ontology/bibo/Book">
        <rdfs:subClassOf rdf:resource="http://purl.org/ontology/bibo/Document"/>
        <rdfs:comment xml:lang="en">A written or printed work of fiction or nonfiction, usually on sheets of paper fastened or bound together within covers.</rdfs:comment>
    </owl:Class>
    


    <!-- http://purl.org/ontology/bibo/BookSection -->

    <owl:Class rdf:about="http://purl.org/ontology/bibo/BookSection">
        <rdfs:subClassOf rdf:resource="http://purl.org/ontology/bibo/DocumentPart"/>
        <rdfs:comment xml:lang="en">A section of a book.</rdfs:comment>
        <rdfs:label xml:lang="en">Book Section</rdfs:label>
    </owl:Class>
    


    <!-- http://purl.org/ontology/bibo/Chapter -->

    <owl:Class rdf:about="http://purl.org/ontology/bibo/Chapter">
        <rdfs:subClassOf rdf:resource="http://purl.org/ontology/bibo/BookSection"/>
        <rdfs:comment xml:lang="en">A chapter of a book.</rdfs:comment>
        <rdfs:label xml:lang="en">Chapter</rdfs:label>
        <skos:AltLabel xml:lang="en">Book chapter</skos:AltLabel>
    </owl:Class>
    


    <!-- http://purl.org/ontology/bibo/CollectedDocument -->

    <owl:Class rdf:about="http://purl.org/ontology/bibo/CollectedDocument">
        <rdfs:subClassOf rdf:resource="http://purl.org/ontology/bibo/Document"/>
        <rdfs:comment xml:lang="en">A document that simultaneously contains other documents.</rdfs:comment>
        <rdfs:label xml:lang="en">Collected Document</rdfs:label>
    </owl:Class>
    


    <!-- http://purl.org/ontology/bibo/Collection -->

    <owl:Class rdf:about="http://purl.org/ontology/bibo/Collection">
        <rdfs:subClassOf rdf:resource="https://www.isibang.ac.in/ns/amv#InformationResource"/>
        <rdfs:comment xml:lang="en">A collection of Documents or Collections.</rdfs:comment>
        <rdfs:label xml:lang="en">Collection</rdfs:label>
    </owl:Class>
    


    <!-- http://purl.org/ontology/bibo/Document -->

    <owl:Class rdf:about="http://purl.org/ontology/bibo/Document">
        <rdfs:subClassOf rdf:resource="https://www.isibang.ac.in/ns/amv#InformationResource"/>
        <rdfs:comment xml:lang="en">A document (noun) is a bounded physical representation of body of information designed with the capacity (and usually intent) to communicate. A document may manifest symbolic, diagrammatic or sensory-representational information.</rdfs:comment>
        <rdfs:comment>The algorithm was published in what kind of literature.</rdfs:comment>
        <rdfs:label xml:lang="en">Document</rdfs:label>
    </owl:Class>
    


    <!-- http://purl.org/ontology/bibo/DocumentPart -->

    <owl:Class rdf:about="http://purl.org/ontology/bibo/DocumentPart">
        <rdfs:subClassOf rdf:resource="http://purl.org/ontology/bibo/Document"/>
        <rdfs:comment xml:lang="en">a distinct part of a larger document or collected document.</rdfs:comment>
        <rdfs:label xml:lang="en">Document Part</rdfs:label>
    </owl:Class>
    


    <!-- http://purl.org/ontology/bibo/EditedBook -->

    <owl:Class rdf:about="http://purl.org/ontology/bibo/EditedBook">
        <rdfs:subClassOf rdf:resource="http://purl.org/ontology/bibo/CollectedDocument"/>
        <rdfs:comment xml:lang="en">An edited book.</rdfs:comment>
        <rdfs:label xml:lang="en">Edited Book</rdfs:label>
    </owl:Class>
    


    <!-- http://purl.org/ontology/bibo/Excerpt -->

    <owl:Class rdf:about="http://purl.org/ontology/bibo/Excerpt">
        <rdfs:subClassOf rdf:resource="http://purl.org/ontology/bibo/DocumentPart"/>
        <rdfs:comment xml:lang="en">A passage selected from a larger work.</rdfs:comment>
        <rdfs:label xml:lang="en">Excerpt</rdfs:label>
    </owl:Class>
    


    <!-- http://purl.org/ontology/bibo/Issue -->

    <owl:Class rdf:about="http://purl.org/ontology/bibo/Issue">
        <rdfs:subClassOf rdf:resource="http://purl.org/ontology/bibo/CollectedDocument"/>
        <rdfs:comment xml:lang="en">something that is printed or published and distributed, esp. a given number of a periodical.</rdfs:comment>
        <rdfs:label xml:lang="en">Issue</rdfs:label>
    </owl:Class>
    


    <!-- http://purl.org/ontology/bibo/Journal -->

    <owl:Class rdf:about="http://purl.org/ontology/bibo/Journal">
        <rdfs:subClassOf rdf:resource="http://purl.org/ontology/bibo/Periodical"/>
        <rdfs:comment xml:lang="en">A periodical of scholarly journal Articles.</rdfs:comment>
        <rdfs:comment xml:lang="en">a periodical dedicated to a particular subject; &quot;he reads the medical journals.&quot;</rdfs:comment>
        <rdfs:label xml:lang="en">Journal</rdfs:label>
    </owl:Class>
    


    <!-- http://purl.org/ontology/bibo/Magazine -->

    <owl:Class rdf:about="http://purl.org/ontology/bibo/Magazine">
        <rdfs:subClassOf rdf:resource="http://purl.org/ontology/bibo/Periodical"/>
        <rdfs:comment xml:lang="en">A periodical of magazine Articles. A magazine is a publication that is issued periodically, usually bound in a paper cover, and typically contains essays, stories, poems, etc., by many writers, and often photographs and drawings, frequently specializing in a particular subject or area, as hobbies, news, or sports.</rdfs:comment>
        <rdfs:comment xml:lang="en">A periodical publication containing articles and illustrations, often on a particular subject or aimed at a particular readership.</rdfs:comment>
        <rdfs:label xml:lang="en">Magazine</rdfs:label>
    </owl:Class>
    


    <!-- http://purl.org/ontology/bibo/Manuscript -->

    <owl:Class rdf:about="http://purl.org/ontology/bibo/Manuscript">
        <rdfs:subClassOf rdf:resource="http://purl.org/ontology/bibo/Document"/>
        <rdfs:comment xml:lang="en">An unpublished Document, which may also be submitted to a publisher for publication.</rdfs:comment>
        <rdfs:label xml:lang="en">Manuscript</rdfs:label>
    </owl:Class>
    


    <!-- http://purl.org/ontology/bibo/Patent -->

    <owl:Class rdf:about="http://purl.org/ontology/bibo/Patent">
        <rdfs:subClassOf rdf:resource="http://purl.org/ontology/bibo/Document"/>
        <rdfs:comment xml:lang="en">A document describing the exclusive right granted by a government to an inventor to manufacture, use, or sell an invention for a certain number of years.</rdfs:comment>
        <rdfs:label xml:lang="en">Patent</rdfs:label>
    </owl:Class>
    


    <!-- http://purl.org/ontology/bibo/Periodical -->

    <owl:Class rdf:about="http://purl.org/ontology/bibo/Periodical">
        <rdfs:subClassOf rdf:resource="http://purl.org/ontology/bibo/Collection"/>
        <rdfs:comment xml:lang="en">A group of related documents issued at regular intervals.</rdfs:comment>
        <rdfs:label xml:lang="en">Priodical</rdfs:label>
    </owl:Class>
    


    <!-- http://purl.org/ontology/bibo/Proceedings -->

    <owl:Class rdf:about="http://purl.org/ontology/bibo/Proceedings">
        <rdfs:subClassOf rdf:resource="http://purl.org/ontology/bibo/Book"/>
        <rdfs:comment xml:lang="en">A compilation of documents published from an event, such as a conference.</rdfs:comment>
        <rdfs:label xml:lang="en">Proceedings</rdfs:label>
    </owl:Class>
    


    <!-- http://purl.org/ontology/bibo/ReferenceSource -->

    <owl:Class rdf:about="http://purl.org/ontology/bibo/ReferenceSource">
        <rdfs:subClassOf rdf:resource="http://purl.org/ontology/bibo/Document"/>
        <rdfs:comment xml:lang="en">A document that presents authoritative reference information, such as a dictionary or encylopedia.</rdfs:comment>
        <rdfs:label xml:lang="en">Reference Source</rdfs:label>
    </owl:Class>
    


    <!-- http://purl.org/ontology/bibo/Report -->

    <owl:Class rdf:about="http://purl.org/ontology/bibo/Report">
        <rdfs:subClassOf rdf:resource="http://purl.org/ontology/bibo/Document"/>
        <rdfs:comment xml:lang="en">A document describing an account or statement describing in detail an event, situation, or the like, usually as the result of observation, inquiry, etc..</rdfs:comment>
        <rdfs:label xml:lang="en">Report</rdfs:label>
    </owl:Class>
    


    <!-- http://purl.org/ontology/bibo/Series -->

    <owl:Class rdf:about="http://purl.org/ontology/bibo/Series">
        <rdfs:subClassOf rdf:resource="http://purl.org/ontology/bibo/Collection"/>
        <rdfs:comment xml:lang="en">A loose, thematic, collection of Documents, often Books.</rdfs:comment>
        <rdfs:label xml:lang="en">Series</rdfs:label>
    </owl:Class>
    


    <!-- http://purl.org/ontology/bibo/Slide -->

    <owl:Class rdf:about="http://purl.org/ontology/bibo/Slide">
        <rdfs:subClassOf rdf:resource="http://purl.org/ontology/bibo/DocumentPart"/>
        <rdfs:comment xml:lang="en">A slide in a slideshow.</rdfs:comment>
        <rdfs:label xml:lang="en">Slide</rdfs:label>
    </owl:Class>
    


    <!-- http://purl.org/ontology/bibo/Thesis -->

    <owl:Class rdf:about="http://purl.org/ontology/bibo/Thesis">
        <rdfs:subClassOf rdf:resource="http://purl.org/ontology/bibo/Document"/>
        <rdfs:comment xml:lang="en">A document created to summarize research findings associated with the completion of an academic degree.</rdfs:comment>
        <rdfs:label xml:lang="en">Thesis</rdfs:label>
    </owl:Class>
    


    <!-- http://purl.org/ontology/bibo/Webpage -->

    <owl:Class rdf:about="http://purl.org/ontology/bibo/Webpage">
        <rdfs:subClassOf rdf:resource="http://purl.org/ontology/bibo/Document"/>
        <rdfs:comment xml:lang="en">A web page is an online document available (at least initially) on the world wide web. A web page is written first and foremost to appear on the web, as distinct from other online resources such as books, manuscripts or audio documents which use the web primarily as a distribution mechanism alongside other more traditional methods such as print.</rdfs:comment>
        <rdfs:label xml:lang="en">Webpage</rdfs:label>
    </owl:Class>
    


    <!-- http://purl.org/ontology/bibo/Website -->

    <owl:Class rdf:about="http://purl.org/ontology/bibo/Website">
        <rdfs:subClassOf rdf:resource="http://purl.org/ontology/bibo/Collection"/>
        <rdfs:comment xml:lang="en">A group of Webpages accessible on the Web.</rdfs:comment>
        <rdfs:label xml:lang="en">Website</rdfs:label>
    </owl:Class>
    


    <!-- http://schema.org/Comment -->

    <owl:Class rdf:about="http://schema.org/Comment">
        <rdfs:comment xml:lang="en">A comment on an item - for example, a comment on a blog post. The comment&apos;s content is expressed via the text property, and its topic via about, properties shared with all CreativeWorks.</rdfs:comment>
        <rdfs:label xml:lang="en">Comment</rdfs:label>
    </owl:Class>
    


    <!-- http://www.wikidata.org/entity/Q8366 -->

    <owl:Class rdf:about="http://www.wikidata.org/entity/Q8366">
        <owl:equivalentClass rdf:resource="https://www.isibang.ac.in/ns/amv#Algorithm"/>
        <rdfs:comment xml:lang="en">Unambiguous specification of how to solve a class of problems.(https://www.wikidata.org/wiki/Q8366)</rdfs:comment>
        <rdfs:label xml:lang="en">Algorithm</rdfs:label>
    </owl:Class>
    


    <!-- http://xmlns.com/foaf/0.1/Agent -->

    <owl:Class rdf:about="http://xmlns.com/foaf/0.1/Agent">
        <rdfs:comment xml:lang="en">A resource that acts or has the power to act. Example of Agents include person and organization.</rdfs:comment>
        <rdfs:label xml:lang="en">Agent</rdfs:label>
    </owl:Class>
    


    <!-- http://xmlns.com/foaf/0.1/Organization -->

    <owl:Class rdf:about="http://xmlns.com/foaf/0.1/Organization">
        <rdfs:subClassOf rdf:resource="http://xmlns.com/foaf/0.1/Agent"/>
        <rdfs:comment xml:lang="en">An agent belonging to some social institutions such as companies, associations etc, that has a collective goal.</rdfs:comment>
        <rdfs:label xml:lang="en">Organization</rdfs:label>
    </owl:Class>
    


    <!-- http://xmlns.com/foaf/0.1/Person -->

    <owl:Class rdf:about="http://xmlns.com/foaf/0.1/Person">
        <rdfs:subClassOf rdf:resource="http://xmlns.com/foaf/0.1/Agent"/>
        <rdfs:comment xml:lang="en">A human.</rdfs:comment>
        <rdfs:label xml:lang="en">Person</rdfs:label>
    </owl:Class>
    


    <!-- https://schema.org/OperatingSystem -->

    <owl:Class rdf:about="https://schema.org/OperatingSystem">
        <rdfs:comment>An Operating System (OS) is an interface between a computer user and computer hardware. An operating system is a software which performs all the basic tasks like file management, memory management, process management, handling input and output, and controlling peripheral devices such as disk drives and printers.</rdfs:comment>
        <rdfs:label xml:lang="en">OperatingSystem</rdfs:label>
    </owl:Class>
    


    <!-- https://www.isibang.ac.in/ns/amv#Algorithm -->

    <owl:Class rdf:about="https://www.isibang.ac.in/ns/amv#Algorithm">
        <rdfs:subClassOf>
            <owl:Restriction>
                <owl:onProperty rdf:resource="http://www.wikidata.org/prop/direct/p2159"/>
                <owl:someValuesFrom rdf:resource="https://www.isibang.ac.in/ns/amv#Problem"/>
            </owl:Restriction>
        </rdfs:subClassOf>
        <rdfs:subClassOf>
            <owl:Restriction>
                <owl:onProperty rdf:resource="https://www.isibang.ac.in/ns/amv#algorithmType"/>
                <owl:someValuesFrom rdf:resource="https://www.isibang.ac.in/ns/amv#AlgorithmicType"/>
            </owl:Restriction>
        </rdfs:subClassOf>
        <rdfs:subClassOf>
            <owl:Restriction>
                <owl:onProperty rdf:resource="https://www.isibang.ac.in/ns/amv#appearedIn"/>
                <owl:someValuesFrom rdf:resource="https://www.isibang.ac.in/ns/amv#InformationResource"/>
            </owl:Restriction>
        </rdfs:subClassOf>
        <rdfs:subClassOf>
            <owl:Restriction>
                <owl:onProperty rdf:resource="https://www.isibang.ac.in/ns/amv#input"/>
                <owl:someValuesFrom rdf:resource="http://www.w3.org/2001/XMLSchema#string"/>
            </owl:Restriction>
        </rdfs:subClassOf>
        <rdfs:subClassOf>
            <owl:Restriction>
                <owl:onProperty rdf:resource="https://www.isibang.ac.in/ns/amv#numberOfSteps"/>
                <owl:someValuesFrom rdf:resource="http://www.w3.org/2001/XMLSchema#nonNegativeInteger"/>
            </owl:Restriction>
        </rdfs:subClassOf>
        <rdfs:subClassOf>
            <owl:Restriction>
                <owl:onProperty rdf:resource="https://www.isibang.ac.in/ns/amv#output"/>
                <owl:someValuesFrom rdf:resource="http://www.w3.org/2001/XMLSchema#string"/>
            </owl:Restriction>
        </rdfs:subClassOf>
        <rdfs:subClassOf>
            <owl:Restriction>
                <owl:onProperty rdf:resource="https://www.isibang.ac.in/ns/amv#spaceComplexity"/>
                <owl:someValuesFrom rdf:resource="http://www.w3.org/2001/XMLSchema#string"/>
            </owl:Restriction>
        </rdfs:subClassOf>
        <rdfs:subClassOf>
            <owl:Restriction>
                <owl:onProperty rdf:resource="https://www.isibang.ac.in/ns/amv#timeComplexity"/>
                <owl:someValuesFrom rdf:resource="http://www.w3.org/2001/XMLSchema#string"/>
            </owl:Restriction>
        </rdfs:subClassOf>
        <rdfs:subClassOf>
            <owl:Restriction>
                <owl:onProperty rdf:resource="http://purl.org/dc/terms/title"/>
                <owl:allValuesFrom rdf:resource="http://www.w3.org/2001/XMLSchema#string"/>
            </owl:Restriction>
        </rdfs:subClassOf>
        <rdfs:subClassOf>
            <owl:Restriction>
                <owl:onProperty rdf:resource="http://purl.org/dc/terms/title"/>
                <owl:minQualifiedCardinality rdf:datatype="http://www.w3.org/2001/XMLSchema#nonNegativeInteger">1</owl:minQualifiedCardinality>
                <owl:onDataRange rdf:resource="http://www.w3.org/2001/XMLSchema#string"/>
            </owl:Restriction>
        </rdfs:subClassOf>
        <rdfs:comment xml:lang="en">It is a finite and unambiguous sequence of computer implementable instructions to perform a certain task. This can be a simple process, such as adding two numbers together, or a complex function, such as adding effects to an image. t can be expressed within a finite amount of space and time and in a well-defined formal language.</rdfs:comment>
        <rdfs:label>Algorithm</rdfs:label>
    </owl:Class>
    


    <!-- https://www.isibang.ac.in/ns/amv#AlgorithmAnalysisFunction -->

    <owl:Class rdf:about="https://www.isibang.ac.in/ns/amv#AlgorithmAnalysisFunction">
        <rdfs:comment xml:lang="en">Time complexity corresponds to the amount of time required for an algorithm to run over the provided input in order to generate the required output. Analysis of this helps to predict the resources that an algorithm will take to finish execution.</rdfs:comment>
        <rdfs:label xml:lang="en">AlgorithmAnalysisFunction</rdfs:label>
    </owl:Class>
    


    <!-- https://www.isibang.ac.in/ns/amv#AlgorithmicType -->

    <owl:Class rdf:about="https://www.isibang.ac.in/ns/amv#AlgorithmicType">
        <rdfs:comment xml:lang="en">The different type of algorithmic techniques that are used to solve the various existing problems in the most optimized manner.</rdfs:comment>
        <rdfs:label xml:lang="en">Algorithmic Type</rdfs:label>
    </owl:Class>
    


    <!-- https://www.isibang.ac.in/ns/amv#CombinatorialProblem -->

    <owl:Class rdf:about="https://www.isibang.ac.in/ns/amv#CombinatorialProblem">
        <rdfs:subClassOf rdf:resource="https://www.isibang.ac.in/ns/amv#Problem"/>
        <rdfs:comment>Combinatorial algorithms are computational procedures which are designed to help solve combinatorial problems. Combinatorial problems are problems involving arrangements of elements from a finite set and selections from a finite set.</rdfs:comment>
        <rdfs:label>Combinatorial Problem</rdfs:label>
    </owl:Class>
    


    <!-- https://www.isibang.ac.in/ns/amv#ComputationalGeometryProblem -->

    <owl:Class rdf:about="https://www.isibang.ac.in/ns/amv#ComputationalGeometryProblem">
        <rdfs:subClassOf rdf:resource="https://www.isibang.ac.in/ns/amv#Problem"/>
        <rdfs:comment>Computational geometry is a branch of computer science devoted to the study of algorithms which can be stated in terms of geometry. Some purely geometrical problems arise out of the study of computational geometric algorithms, and such problems are also considered to be part of computational geometry.</rdfs:comment>
        <rdfs:label>ComputationalGeometryProblem</rdfs:label>
    </owl:Class>
    


    <!-- https://www.isibang.ac.in/ns/amv#DataStructure -->

    <owl:Class rdf:about="https://www.isibang.ac.in/ns/amv#DataStructure">
        <rdfs:comment xml:lang="en">A data structure is a named location that can be used to store and organize data.</rdfs:comment>
        <rdfs:label>Data Structure</rdfs:label>
    </owl:Class>
    


    <!-- https://www.isibang.ac.in/ns/amv#DataStructuresProblem -->

    <owl:Class rdf:about="https://www.isibang.ac.in/ns/amv#DataStructuresProblem">
        <rdfs:subClassOf rdf:resource="https://www.isibang.ac.in/ns/amv#Problem"/>
        <rdfs:comment>Solving problems related to data structure i.e  a particular way of organizing data in a computer so that it can be used effectively.</rdfs:comment>
        <rdfs:label>DataStructuresProblem</rdfs:label>
    </owl:Class>
    


    <!-- https://www.isibang.ac.in/ns/amv#FormOfExpression -->

    <owl:Class rdf:about="https://www.isibang.ac.in/ns/amv#FormOfExpression">
        <rdfs:comment xml:lang="en">The available form of expression/ notation of an algorithm. For example, Flowcharts, pseudocode, control tables, etc. (source: https://en.wikipedia.org/wiki/Algorithm)</rdfs:comment>
        <rdfs:label xml:lang="en">Form of expression</rdfs:label>
    </owl:Class>
    


    <!-- https://www.isibang.ac.in/ns/amv#GraphProblem -->

    <owl:Class rdf:about="https://www.isibang.ac.in/ns/amv#GraphProblem">
        <rdfs:subClassOf rdf:resource="https://www.isibang.ac.in/ns/amv#Problem"/>
        <rdfs:comment>A Graph is a non-linear data structure consisting of nodes and edges. The nodes are sometimes also referred to as vertices and the edges are lines or arcs that connect any two nodes in the graph.</rdfs:comment>
        <rdfs:label>GraphProblem</rdfs:label>
    </owl:Class>
    


    <!-- https://www.isibang.ac.in/ns/amv#HardProblem -->

    <owl:Class rdf:about="https://www.isibang.ac.in/ns/amv#HardProblem">
        <rdfs:subClassOf rdf:resource="https://www.isibang.ac.in/ns/amv#GraphProblem"/>
        <rdfs:comment>Any graph problem, which is NP-hard in general graphs, becomes polynomial-time solvable when restricted to graphs in special
classes.</rdfs:comment>
        <rdfs:label>HardProblem</rdfs:label>
    </owl:Class>
    


    <!-- https://www.isibang.ac.in/ns/amv#Implementation -->

    <owl:Class rdf:about="https://www.isibang.ac.in/ns/amv#Implementation">
        <rdfs:subClassOf rdf:resource="https://www.isibang.ac.in/ns/amv#realizableEntity"/>
        <rdfs:subClassOf>
            <owl:Restriction>
                <owl:onProperty rdf:resource="https://www.isibang.ac.in/ns/amv#implementationInLanguage"/>
                <owl:someValuesFrom rdf:resource="https://www.wikidata.org/wiki/Q9143#ProgrammingLanguage"/>
            </owl:Restriction>
        </rdfs:subClassOf>
        <rdfs:subClassOf>
            <owl:Restriction>
                <owl:onProperty rdf:resource="https://www.isibang.ac.in/ns/amv#isImplementationOf"/>
                <owl:someValuesFrom rdf:resource="https://www.isibang.ac.in/ns/amv#Algorithm"/>
            </owl:Restriction>
        </rdfs:subClassOf>
        <rdfs:subClassOf>
            <owl:Restriction>
                <owl:onProperty rdf:resource="https://www.isibang.ac.in/ns/amv#runsOnOperatingSystem"/>
                <owl:someValuesFrom rdf:resource="https://schema.org/OperatingSystem"/>
            </owl:Restriction>
        </rdfs:subClassOf>
        <rdfs:comment xml:lang="en">A manifestation of a technical specification or algorithm as a program, software component, or other computer system through computer programming and deployment (source: https://en.wikipedia.org/wiki/Implementation).</rdfs:comment>
        <rdfs:label xml:lang="en">Implementation</rdfs:label>
    </owl:Class>
    


    <!-- https://www.isibang.ac.in/ns/amv#InformationResource -->

    <owl:Class rdf:about="https://www.isibang.ac.in/ns/amv#InformationResource">
        <rdfs:comment xml:lang="en">An information resource.</rdfs:comment>
        <rdfs:label xml:lang="en">Information Resource</rdfs:label>
    </owl:Class>
    


    <!-- https://www.isibang.ac.in/ns/amv#LoopConstruct -->

    <owl:Class rdf:about="https://www.isibang.ac.in/ns/amv#LoopConstruct">
        <rdfs:comment xml:lang="en">The type of loop best suited when an algorithm is implemented in any desired programming language. The loop types are for loop, while loop, do-while loop.</rdfs:comment>
        <rdfs:label xml:lang="en">LoopType</rdfs:label>
    </owl:Class>
    


    <!-- https://www.isibang.ac.in/ns/amv#Manual -->

    <owl:Class rdf:about="https://www.isibang.ac.in/ns/amv#Manual">
        <rdfs:subClassOf rdf:resource="http://purl.org/ontology/bibo/Document"/>
        <rdfs:comment xml:lang="en">A small reference book, especially one giving instructions.</rdfs:comment>
        <rdfs:label xml:lang="en">Manual</rdfs:label>
    </owl:Class>
    


    <!-- https://www.isibang.ac.in/ns/amv#Mathematical_Properties -->

    <owl:Class rdf:about="https://www.isibang.ac.in/ns/amv#Mathematical_Properties">
        <rdfs:comment xml:lang="en">The mathematical concept used in the algorithm to tackle the problem. This includes set theoty, linear algebra, graph theory etc.</rdfs:comment>
        <rdfs:label xml:lang="en">MathematicalProperty</rdfs:label>
    </owl:Class>
    


    <!-- https://www.isibang.ac.in/ns/amv#NumericalProblem -->

    <owl:Class rdf:about="https://www.isibang.ac.in/ns/amv#NumericalProblem">
        <rdfs:subClassOf rdf:resource="https://www.isibang.ac.in/ns/amv#Problem"/>
        <rdfs:comment>Numerical algorithms are behind designing shapes (e.g. shapes for cars, planes, fonts), computing intensities for displaying graphics, animating moving objects, studying the spread of diseases, modelling the orbit of planets and satellites, supporting search engines such as google, and many more practical problems.</rdfs:comment>
        <rdfs:label>NumericalProblem</rdfs:label>
    </owl:Class>
    


    <!-- https://www.isibang.ac.in/ns/amv#PolynomialTimeProblem -->

    <owl:Class rdf:about="https://www.isibang.ac.in/ns/amv#PolynomialTimeProblem">
        <rdfs:subClassOf rdf:resource="https://www.isibang.ac.in/ns/amv#GraphProblem"/>
        <rdfs:comment>Polynomial time problem means which means that an algorithm exists for its solution such that the number of steps in the algorithm is bounded by a polynomial function of n, where n corresponds to the length of the input for the problem.</rdfs:comment>
        <rdfs:label>PolynomialTimeProblem</rdfs:label>
    </owl:Class>
    


    <!-- https://www.isibang.ac.in/ns/amv#Problem -->

    <owl:Class rdf:about="https://www.isibang.ac.in/ns/amv#Problem">
        <rdfs:comment xml:lang="en">The various problems for which an algorithm is written.</rdfs:comment>
        <rdfs:label xml:lang="en">Problem</rdfs:label>
    </owl:Class>
    


    <!-- https://www.isibang.ac.in/ns/amv#SetAndStringProblem -->

    <owl:Class rdf:about="https://www.isibang.ac.in/ns/amv#SetAndStringProblem">
        <rdfs:subClassOf rdf:resource="https://www.isibang.ac.in/ns/amv#Problem"/>
        <rdfs:comment>Sets and strings both represent collections of objectsthe difference is whether order matters.Sets are collections of symbols whose order is assumed to carry no significance, while strings are defined by the sequence or arrangement of symbols.</rdfs:comment>
        <rdfs:label>SetAndStringProblem</rdfs:label>
    </owl:Class>
    


    <!-- https://www.isibang.ac.in/ns/amv#realizableEntity -->

    <owl:Class rdf:about="https://www.isibang.ac.in/ns/amv#realizableEntity">
        <rdfs:comment xml:lang="en">A manifested, actualized and extended form of an idea. For example, a software code is a manifestation and actualization of an algorithm. The function or purpose of an algorithm is realized through the actual software code running on a computer.</rdfs:comment>
        <rdfs:label xml:lang="en">Realizable entity</rdfs:label>
        <skos:AltLabel xml:lang="en">Mind product</skos:AltLabel>
    </owl:Class>
    


    <!-- https://www.wikidata.org/wiki/Q11862829 -->

    <owl:Class rdf:about="https://www.wikidata.org/wiki/Q11862829">
        <rdfs:comment xml:lang="en">An area of knowledge or a flield of study that an algorithm deals with.</rdfs:comment>
        <rdfs:label xml:lang="en">Academic discipline</rdfs:label>
    </owl:Class>
    


    <!-- https://www.wikidata.org/wiki/Q9143#ProgrammingLanguage -->

    <owl:Class rdf:about="https://www.wikidata.org/wiki/Q9143#ProgrammingLanguage">
        <rdfs:comment>Language designed to communicate instructions to a machine Programming languages are used in computer programming to implement algorithms.</rdfs:comment>
        <rdfs:label xml:lang="en">ProgrammingLanguage</rdfs:label>
    </owl:Class>
    


    <!-- 
    ///////////////////////////////////////////////////////////////////////////////////////
    //
    // Individuals
    //
    ///////////////////////////////////////////////////////////////////////////////////////
     -->

    


    <!-- https://www.isibang.ac.in/ns/GeneralAlgebra -->

    <owl:NamedIndividual rdf:about="https://www.isibang.ac.in/ns/GeneralAlgebra">
        <rdf:type rdf:resource="https://www.isibang.ac.in/ns/amv#Mathematical_Properties"/>
    </owl:NamedIndividual>
    


    <!-- https://www.isibang.ac.in/ns/amv#Ada -->

    <owl:NamedIndividual rdf:about="https://www.isibang.ac.in/ns/amv#Ada">
        <rdf:type rdf:resource="https://www.wikidata.org/wiki/Q9143#ProgrammingLanguage"/>
    </owl:NamedIndividual>
    


    <!-- https://www.isibang.ac.in/ns/amv#Apache -->

    <owl:NamedIndividual rdf:about="https://www.isibang.ac.in/ns/amv#Apache">
        <rdf:type rdf:resource="http://purl.org/dc/terms/LicenseDocument"/>
    </owl:NamedIndividual>
    


    <!-- https://www.isibang.ac.in/ns/amv#Array -->

    <owl:NamedIndividual rdf:about="https://www.isibang.ac.in/ns/amv#Array">
        <rdf:type rdf:resource="https://www.isibang.ac.in/ns/amv#DataStructure"/>
    </owl:NamedIndividual>
    


    <!-- https://www.isibang.ac.in/ns/amv#BSDSort -->

    <owl:NamedIndividual rdf:about="https://www.isibang.ac.in/ns/amv#BSDSort">
        <rdf:type rdf:resource="https://www.isibang.ac.in/ns/amv#Implementation"/>
        <terms:contributor rdf:resource="https://www.isibang.ac.in/ns/amv#JaromirDolecek"/>
        <terms:creator rdf:resource="https://www.isibang.ac.in/ns/amv#PeterMcIlroy"/>
        <isImplementationOf rdf:resource="https://www.isibang.ac.in/ns/amv#SortUnix"/>
        <runsOnOperatingSystem rdf:resource="https://www.isibang.ac.in/ns/amv#Unix"/>
        <terms:date rdf:datatype="http://www.w3.org/2001/XMLSchema#dateTime">2001-01-01T00:00:00</terms:date>
        <terms:description rdf:datatype="http://www.w3.org/2001/XMLSchema#string">BSD sort is BSD-licenced implementation if Unix(TM) sort(1) utility. Feature wise, it&apos;s on-par with GNU sort(1), but is faster and smaller. BSD sort(1) uses radixsort(3) as the core of the sorting functionality itself.</terms:description>
        <terms:identifier rdf:datatype="http://www.w3.org/2001/XMLSchema#anyURI">http://bsdsort.sourceforge.net/</terms:identifier>
    </owl:NamedIndividual>
    


    <!-- https://www.isibang.ac.in/ns/amv#BacktrackingAlgorithm -->

    <owl:NamedIndividual rdf:about="https://www.isibang.ac.in/ns/amv#BacktrackingAlgorithm">
        <rdf:type rdf:resource="https://www.isibang.ac.in/ns/amv#AlgorithmicType"/>
    </owl:NamedIndividual>
    


    <!-- https://www.isibang.ac.in/ns/amv#BandwidthReduction -->

    <owl:NamedIndividual rdf:about="https://www.isibang.ac.in/ns/amv#BandwidthReduction">
        <rdf:type rdf:resource="https://www.isibang.ac.in/ns/amv#NumericalProblem"/>
    </owl:NamedIndividual>
    


    <!-- https://www.isibang.ac.in/ns/amv#Basic -->

    <owl:NamedIndividual rdf:about="https://www.isibang.ac.in/ns/amv#Basic">
        <rdf:type rdf:resource="https://www.wikidata.org/wiki/Q9143#ProgrammingLanguage"/>
    </owl:NamedIndividual>
    


    <!-- https://www.isibang.ac.in/ns/amv#BinarySearchAlgorithm -->

    <owl:NamedIndividual rdf:about="https://www.isibang.ac.in/ns/amv#BinarySearchAlgorithm">
        <rdf:type rdf:resource="https://www.isibang.ac.in/ns/amv#Algorithm"/>
        <terms:creator rdf:resource="https://www.isibang.ac.in/ns/amv#DerrickHenryLehmer"/>
        <terms:creator rdf:resource="https://www.isibang.ac.in/ns/amv#JohnMauchly"/>
        <terms:creator rdf:resource="https://www.isibang.ac.in/ns/amv#WilliamWesleyPeterson"/>
        <terms:subject rdf:resource="https://www.isibang.ac.in/ns/amv#ComputerScience"/>
        <wdt:p2159 rdf:resource="https://www.isibang.ac.in/ns/amv#Searching"/>
        <algorithmAnalysisFunctionType rdf:resource="https://www.isibang.ac.in/ns/amv#LogarithmicFunction"/>
        <algorithmType rdf:resource="https://www.isibang.ac.in/ns/amv#DivideAndConquerAlgorithm"/>
        <dataStructureUsed rdf:resource="https://www.isibang.ac.in/ns/amv#Array"/>
        <terms:created rdf:datatype="http://www.w3.org/2001/XMLSchema#dateTime">1960-01-01T00:00:00</terms:created>
        <terms:description rdf:datatype="http://www.w3.org/2001/XMLSchema#string">Binary search is a search algorithm that finds the position of a target value within a sorted array. Binary search compares the target value to the middle element of the array. If they are not equal, the half in which the target cannot lie is eliminated and the search continues on the remaining half, again taking the middle element to compare to the target value, and repeating this until the target value is found. If the search ends with the remaining half being empty, the target is not in the array.
-https://en.wikipedia.org/wiki/Binary_search_algorithm</terms:description>
        <terms:title>BinarySearch</terms:title>
        <wdt:P3752 rdf:datatype="http://www.w3.org/2001/XMLSchema#string">O(log n)</wdt:P3752>
        <wdt:P3753 rdf:datatype="http://www.w3.org/2001/XMLSchema#string">O(1)</wdt:P3753>
        <wdt:P3754 rdf:datatype="http://www.w3.org/2001/XMLSchema#string">O(log n)</wdt:P3754>
        <Constraint rdf:datatype="http://www.w3.org/2001/XMLSchema#string">Binary search can only be done on sorted array.</Constraint>
        <edgeCase rdf:datatype="http://www.w3.org/2001/XMLSchema#string">A binary search works by &quot;cutting the search space in half&quot;, but actual implementation might have an edge case when the element you&apos;re looking for is right in the middle of the search space, or if the number of elements is even and there is technically no &quot;middle&quot; element</edgeCase>
        <numberOfSteps rdf:datatype="http://www.w3.org/2001/XMLSchema#integer">4</numberOfSteps>
    </owl:NamedIndividual>
    <owl:Axiom>
        <owl:annotatedSource rdf:resource="https://www.isibang.ac.in/ns/amv#BinarySearchAlgorithm"/>
        <owl:annotatedProperty rdf:resource="http://www.w3.org/1999/02/22-rdf-syntax-ns#type"/>
        <owl:annotatedTarget rdf:resource="https://www.isibang.ac.in/ns/amv#Algorithm"/>
        <rdfs:comment rdf:resource="https://www.isibang.ac.in/ns/amv#creator"/>
    </owl:Axiom>
    


    <!-- https://www.isibang.ac.in/ns/amv#BranchAndBoundAlgorithm -->

    <owl:NamedIndividual rdf:about="https://www.isibang.ac.in/ns/amv#BranchAndBoundAlgorithm">
        <rdf:type rdf:resource="https://www.isibang.ac.in/ns/amv#AlgorithmicType"/>
    </owl:NamedIndividual>
    


    <!-- https://www.isibang.ac.in/ns/amv#BruteForceAlgorithm -->

    <owl:NamedIndividual rdf:about="https://www.isibang.ac.in/ns/amv#BruteForceAlgorithm">
        <rdf:type rdf:resource="https://www.isibang.ac.in/ns/amv#AlgorithmicType"/>
    </owl:NamedIndividual>
    


    <!-- https://www.isibang.ac.in/ns/amv#C -->

    <owl:NamedIndividual rdf:about="https://www.isibang.ac.in/ns/amv#C">
        <rdf:type rdf:resource="https://www.wikidata.org/wiki/Q9143#ProgrammingLanguage"/>
    </owl:NamedIndividual>
    


    <!-- https://www.isibang.ac.in/ns/amv#ComputerScience -->

    <owl:NamedIndividual rdf:about="https://www.isibang.ac.in/ns/amv#ComputerScience">
        <rdf:type rdf:resource="https://www.wikidata.org/wiki/Q11862829"/>
    </owl:NamedIndividual>
    


    <!-- https://www.isibang.ac.in/ns/amv#ConnectedComponents -->

    <owl:NamedIndividual rdf:about="https://www.isibang.ac.in/ns/amv#ConnectedComponents">
        <rdf:type rdf:resource="https://www.isibang.ac.in/ns/amv#PolynomialTimeProblem"/>
    </owl:NamedIndividual>
    


    <!-- https://www.isibang.ac.in/ns/amv#ConstantFunctions -->

    <owl:NamedIndividual rdf:about="https://www.isibang.ac.in/ns/amv#ConstantFunctions">
        <rdf:type rdf:resource="https://www.isibang.ac.in/ns/amv#AlgorithmAnalysisFunction"/>
    </owl:NamedIndividual>
    


    <!-- https://www.isibang.ac.in/ns/amv#ControlTable -->

    <owl:NamedIndividual rdf:about="https://www.isibang.ac.in/ns/amv#ControlTable">
        <rdf:type rdf:resource="https://www.isibang.ac.in/ns/amv#FormOfExpression"/>
    </owl:NamedIndividual>
    


    <!-- https://www.isibang.ac.in/ns/amv#ConvexHull -->

    <owl:NamedIndividual rdf:about="https://www.isibang.ac.in/ns/amv#ConvexHull">
        <rdf:type rdf:resource="https://www.isibang.ac.in/ns/amv#ComputationalGeometryProblem"/>
    </owl:NamedIndividual>
    


    <!-- https://www.isibang.ac.in/ns/amv#Copyleft -->

    <owl:NamedIndividual rdf:about="https://www.isibang.ac.in/ns/amv#Copyleft">
        <rdf:type rdf:resource="http://purl.org/dc/terms/LicenseDocument"/>
    </owl:NamedIndividual>
    


    <!-- https://www.isibang.ac.in/ns/amv#CreativeCommonsAttribution3.0 -->

    <owl:NamedIndividual rdf:about="https://www.isibang.ac.in/ns/amv#CreativeCommonsAttribution3.0">
        <rdf:type rdf:resource="http://purl.org/dc/terms/LicenseDocument"/>
    </owl:NamedIndividual>
    


    <!-- https://www.isibang.ac.in/ns/amv#CreativeCommonsAttribution4.0 -->

    <owl:NamedIndividual rdf:about="https://www.isibang.ac.in/ns/amv#CreativeCommonsAttribution4.0">
        <rdf:type rdf:resource="http://purl.org/dc/terms/LicenseDocument"/>
    </owl:NamedIndividual>
    


    <!-- https://www.isibang.ac.in/ns/amv#Cryptography -->

    <owl:NamedIndividual rdf:about="https://www.isibang.ac.in/ns/amv#Cryptography">
        <rdf:type rdf:resource="https://www.isibang.ac.in/ns/amv#SetAndStringProblem"/>
    </owl:NamedIndividual>
    


    <!-- https://www.isibang.ac.in/ns/amv#CubicFunctionsAndPolynomials -->

    <owl:NamedIndividual rdf:about="https://www.isibang.ac.in/ns/amv#CubicFunctionsAndPolynomials">
        <rdf:type rdf:resource="https://www.isibang.ac.in/ns/amv#AlgorithmAnalysisFunction"/>
    </owl:NamedIndividual>
    


    <!-- https://www.isibang.ac.in/ns/amv#DelbertRayFulkerson -->

    <owl:NamedIndividual rdf:about="https://www.isibang.ac.in/ns/amv#DelbertRayFulkerson">
        <rdf:type rdf:resource="http://xmlns.com/foaf/0.1/Person"/>
    </owl:NamedIndividual>
    


    <!-- https://www.isibang.ac.in/ns/amv#Department -->

    <owl:NamedIndividual rdf:about="https://www.isibang.ac.in/ns/amv#Department">
        <rdf:type rdf:resource="http://purl.org/dc/terms/RightsStatement"/>
    </owl:NamedIndividual>
    


    <!-- https://www.isibang.ac.in/ns/amv#DerrickHenryLehmer -->

    <owl:NamedIndividual rdf:about="https://www.isibang.ac.in/ns/amv#DerrickHenryLehmer">
        <rdf:type rdf:resource="http://xmlns.com/foaf/0.1/Person"/>
    </owl:NamedIndividual>
    


    <!-- https://www.isibang.ac.in/ns/amv#DeterminantsAndPermanents -->

    <owl:NamedIndividual rdf:about="https://www.isibang.ac.in/ns/amv#DeterminantsAndPermanents">
        <rdf:type rdf:resource="https://www.isibang.ac.in/ns/amv#NumericalProblem"/>
    </owl:NamedIndividual>
    


    <!-- https://www.isibang.ac.in/ns/amv#Dictionaries -->

    <owl:NamedIndividual rdf:about="https://www.isibang.ac.in/ns/amv#Dictionaries">
        <rdf:type rdf:resource="https://www.isibang.ac.in/ns/amv#DataStructuresProblem"/>
    </owl:NamedIndividual>
    


    <!-- https://www.isibang.ac.in/ns/amv#Dictionary -->

    <owl:NamedIndividual rdf:about="https://www.isibang.ac.in/ns/amv#Dictionary">
        <rdf:type rdf:resource="https://www.isibang.ac.in/ns/amv#DataStructure"/>
    </owl:NamedIndividual>
    


    <!-- https://www.isibang.ac.in/ns/amv#DifferentialCalculus -->

    <owl:NamedIndividual rdf:about="https://www.isibang.ac.in/ns/amv#DifferentialCalculus">
        <rdf:type rdf:resource="https://www.isibang.ac.in/ns/amv#Mathematical_Properties"/>
    </owl:NamedIndividual>
    


    <!-- https://www.isibang.ac.in/ns/amv#DivideAndConquerAlgorithm -->

    <owl:NamedIndividual rdf:about="https://www.isibang.ac.in/ns/amv#DivideAndConquerAlgorithm">
        <rdf:type rdf:resource="https://www.isibang.ac.in/ns/amv#AlgorithmicType"/>
    </owl:NamedIndividual>
    


    <!-- https://www.isibang.ac.in/ns/amv#DoWhile -->

    <owl:NamedIndividual rdf:about="https://www.isibang.ac.in/ns/amv#DoWhile">
        <rdf:type rdf:resource="https://www.isibang.ac.in/ns/amv#LoopConstruct"/>
    </owl:NamedIndividual>
    


    <!-- https://www.isibang.ac.in/ns/amv#DonaldKnuth -->

    <owl:NamedIndividual rdf:about="https://www.isibang.ac.in/ns/amv#DonaldKnuth">
        <rdf:type rdf:resource="http://xmlns.com/foaf/0.1/Person"/>
    </owl:NamedIndividual>
    


    <!-- https://www.isibang.ac.in/ns/amv#Drakon-chart -->

    <owl:NamedIndividual rdf:about="https://www.isibang.ac.in/ns/amv#Drakon-chart">
        <rdf:type rdf:resource="https://www.isibang.ac.in/ns/amv#FormOfExpression"/>
    </owl:NamedIndividual>
    


    <!-- https://www.isibang.ac.in/ns/amv#DynamicProgrammingAlgorithm -->

    <owl:NamedIndividual rdf:about="https://www.isibang.ac.in/ns/amv#DynamicProgrammingAlgorithm">
        <rdf:type rdf:resource="https://www.isibang.ac.in/ns/amv#AlgorithmicType"/>
    </owl:NamedIndividual>
    


    <!-- https://www.isibang.ac.in/ns/amv#EdgeColoring -->

    <owl:NamedIndividual rdf:about="https://www.isibang.ac.in/ns/amv#EdgeColoring">
        <rdf:type rdf:resource="https://www.isibang.ac.in/ns/amv#HardProblem"/>
    </owl:NamedIndividual>
    


    <!-- https://www.isibang.ac.in/ns/amv#EdouardLucas -->

    <owl:NamedIndividual rdf:about="https://www.isibang.ac.in/ns/amv#EdouardLucas">
        <rdf:type rdf:resource="http://xmlns.com/foaf/0.1/Person"/>
    </owl:NamedIndividual>
    


    <!-- https://www.isibang.ac.in/ns/amv#EdwardWForgy -->

    <owl:NamedIndividual rdf:about="https://www.isibang.ac.in/ns/amv#EdwardWForgy">
        <rdf:type rdf:resource="http://xmlns.com/foaf/0.1/Person"/>
    </owl:NamedIndividual>
    


    <!-- https://www.isibang.ac.in/ns/amv#ExponentialFunctions -->

    <owl:NamedIndividual rdf:about="https://www.isibang.ac.in/ns/amv#ExponentialFunctions">
        <rdf:type rdf:resource="https://www.isibang.ac.in/ns/amv#AlgorithmAnalysisFunction"/>
    </owl:NamedIndividual>
    


    <!-- https://www.isibang.ac.in/ns/amv#Flowchart -->

    <owl:NamedIndividual rdf:about="https://www.isibang.ac.in/ns/amv#Flowchart">
        <rdf:type rdf:resource="https://www.isibang.ac.in/ns/amv#FormOfExpression"/>
    </owl:NamedIndividual>
    


    <!-- https://www.isibang.ac.in/ns/amv#For -->

    <owl:NamedIndividual rdf:about="https://www.isibang.ac.in/ns/amv#For">
        <rdf:type rdf:resource="https://www.isibang.ac.in/ns/amv#LoopConstruct"/>
    </owl:NamedIndividual>
    


    <!-- https://www.isibang.ac.in/ns/amv#Fortran -->

    <owl:NamedIndividual rdf:about="https://www.isibang.ac.in/ns/amv#Fortran">
        <rdf:type rdf:resource="https://www.wikidata.org/wiki/Q9143#ProgrammingLanguage"/>
    </owl:NamedIndividual>
    


    <!-- https://www.isibang.ac.in/ns/amv#GNU -->

    <owl:NamedIndividual rdf:about="https://www.isibang.ac.in/ns/amv#GNU">
        <rdf:type rdf:resource="http://purl.org/dc/terms/LicenseDocument"/>
    </owl:NamedIndividual>
    


    <!-- https://www.isibang.ac.in/ns/amv#GPL -->

    <owl:NamedIndividual rdf:about="https://www.isibang.ac.in/ns/amv#GPL">
        <rdf:type rdf:resource="http://purl.org/dc/terms/LicenseDocument"/>
    </owl:NamedIndividual>
    


    <!-- https://www.isibang.ac.in/ns/amv#GaussianElimination -->

    <owl:NamedIndividual rdf:about="https://www.isibang.ac.in/ns/amv#GaussianElimination">
        <rdf:type rdf:resource="https://www.isibang.ac.in/ns/amv#Mathematical_Properties"/>
    </owl:NamedIndividual>
    


    <!-- https://www.isibang.ac.in/ns/amv#GeneratingGraphs -->

    <owl:NamedIndividual rdf:about="https://www.isibang.ac.in/ns/amv#GeneratingGraphs">
        <rdf:type rdf:resource="https://www.isibang.ac.in/ns/amv#CombinatorialProblem"/>
    </owl:NamedIndividual>
    


    <!-- https://www.isibang.ac.in/ns/amv#GeneratingSubsets -->

    <owl:NamedIndividual rdf:about="https://www.isibang.ac.in/ns/amv#GeneratingSubsets">
        <rdf:type rdf:resource="https://www.isibang.ac.in/ns/amv#CombinatorialProblem"/>
    </owl:NamedIndividual>
    


    <!-- https://www.isibang.ac.in/ns/amv#GeorgeDantzig -->

    <owl:NamedIndividual rdf:about="https://www.isibang.ac.in/ns/amv#GeorgeDantzig">
        <rdf:type rdf:resource="http://xmlns.com/foaf/0.1/Person"/>
    </owl:NamedIndividual>
    


    <!-- https://www.isibang.ac.in/ns/amv#Graph -->

    <owl:NamedIndividual rdf:about="https://www.isibang.ac.in/ns/amv#Graph">
        <rdf:type rdf:resource="https://www.wikidata.org/wiki/Q11862829"/>
    </owl:NamedIndividual>
    


    <!-- https://www.isibang.ac.in/ns/amv#GraphDataStructures -->

    <owl:NamedIndividual rdf:about="https://www.isibang.ac.in/ns/amv#GraphDataStructures">
        <rdf:type rdf:resource="https://www.isibang.ac.in/ns/amv#DataStructuresProblem"/>
    </owl:NamedIndividual>
    


    <!-- https://www.isibang.ac.in/ns/amv#GraphPartition -->

    <owl:NamedIndividual rdf:about="https://www.isibang.ac.in/ns/amv#GraphPartition">
        <rdf:type rdf:resource="https://www.isibang.ac.in/ns/amv#HardProblem"/>
    </owl:NamedIndividual>
    


    <!-- https://www.isibang.ac.in/ns/amv#GraphTheory -->

    <owl:NamedIndividual rdf:about="https://www.isibang.ac.in/ns/amv#GraphTheory">
        <rdf:type rdf:resource="https://www.isibang.ac.in/ns/amv#Mathematical_Properties"/>
    </owl:NamedIndividual>
    


    <!-- https://www.isibang.ac.in/ns/amv#GreedyAlgorithm -->

    <owl:NamedIndividual rdf:about="https://www.isibang.ac.in/ns/amv#GreedyAlgorithm">
        <rdf:type rdf:resource="https://www.isibang.ac.in/ns/amv#AlgorithmicType"/>
    </owl:NamedIndividual>
    


    <!-- https://www.isibang.ac.in/ns/amv#HamiltonianCycle -->

    <owl:NamedIndividual rdf:about="https://www.isibang.ac.in/ns/amv#HamiltonianCycle">
        <rdf:type rdf:resource="https://www.isibang.ac.in/ns/amv#HardProblem"/>
    </owl:NamedIndividual>
    


    <!-- https://www.isibang.ac.in/ns/amv#HashTable -->

    <owl:NamedIndividual rdf:about="https://www.isibang.ac.in/ns/amv#HashTable">
        <rdf:type rdf:resource="https://www.isibang.ac.in/ns/amv#DataStructure"/>
    </owl:NamedIndividual>
    


    <!-- https://www.isibang.ac.in/ns/amv#IndependentSet -->

    <owl:NamedIndividual rdf:about="https://www.isibang.ac.in/ns/amv#IndependentSet">
        <rdf:type rdf:resource="https://www.isibang.ac.in/ns/amv#HardProblem"/>
    </owl:NamedIndividual>
    


    <!-- https://www.isibang.ac.in/ns/amv#InsertionSortAlgorithm -->

    <owl:NamedIndividual rdf:about="https://www.isibang.ac.in/ns/amv#InsertionSortAlgorithm">
        <rdf:type rdf:resource="https://www.isibang.ac.in/ns/amv#Algorithm"/>
        <terms:creator rdf:resource="https://www.isibang.ac.in/ns/amv#JohnMauchly"/>
        <terms:subject rdf:resource="https://www.isibang.ac.in/ns/amv#ComputerScience"/>
        <algorithmAnalysisFunctionType rdf:resource="https://www.isibang.ac.in/ns/amv#ExponentialFunctions"/>
        <algorithmType rdf:resource="https://www.isibang.ac.in/ns/amv#BruteForceAlgorithm"/>
        <dataStructureUsed rdf:resource="https://www.isibang.ac.in/ns/amv#Array"/>
        <terms:created rdf:datatype="http://www.w3.org/2001/XMLSchema#dateTime">1946-01-01T00:00:00</terms:created>
        <terms:title rdf:datatype="http://www.w3.org/2001/XMLSchema#string">InsertionSort</terms:title>
        <wdt:P3752>O(n^2)</wdt:P3752>
        <wdt:P3753 rdf:datatype="http://www.w3.org/2001/XMLSchema#string">O(n)</wdt:P3753>
        <wdt:P3754>O(n^2)</wdt:P3754>
        <Readable rdf:datatype="http://www.w3.org/2001/XMLSchema#boolean">true</Readable>
        <input rdf:datatype="http://www.w3.org/2001/XMLSchema#string">an array of numbers</input>
        <numberOfSteps rdf:datatype="http://www.w3.org/2001/XMLSchema#integer">6</numberOfSteps>
        <onlineAlgorithm rdf:datatype="http://www.w3.org/2001/XMLSchema#boolean">true</onlineAlgorithm>
    </owl:NamedIndividual>
    


    <!-- https://www.isibang.ac.in/ns/amv#Internal -->

    <owl:NamedIndividual rdf:about="https://www.isibang.ac.in/ns/amv#Internal">
        <rdf:type rdf:resource="http://purl.org/dc/terms/RightsStatement"/>
    </owl:NamedIndividual>
    


    <!-- https://www.isibang.ac.in/ns/amv#JHHalton -->

    <owl:NamedIndividual rdf:about="https://www.isibang.ac.in/ns/amv#JHHalton">
        <rdf:type rdf:resource="http://xmlns.com/foaf/0.1/Person"/>
    </owl:NamedIndividual>
    


    <!-- https://www.isibang.ac.in/ns/amv#JamesHMorris -->

    <owl:NamedIndividual rdf:about="https://www.isibang.ac.in/ns/amv#JamesHMorris">
        <rdf:type rdf:resource="http://xmlns.com/foaf/0.1/Person"/>
    </owl:NamedIndividual>
    


    <!-- https://www.isibang.ac.in/ns/amv#JaromirDolecek -->

    <owl:NamedIndividual rdf:about="https://www.isibang.ac.in/ns/amv#JaromirDolecek"/>
    


    <!-- https://www.isibang.ac.in/ns/amv#Java -->

    <owl:NamedIndividual rdf:about="https://www.isibang.ac.in/ns/amv#Java">
        <rdf:type rdf:resource="https://www.wikidata.org/wiki/Q9143#ProgrammingLanguage"/>
    </owl:NamedIndividual>
    


    <!-- https://www.isibang.ac.in/ns/amv#JillianBeardwood -->

    <owl:NamedIndividual rdf:about="https://www.isibang.ac.in/ns/amv#JillianBeardwood">
        <rdf:type rdf:resource="http://xmlns.com/foaf/0.1/Person"/>
    </owl:NamedIndividual>
    


    <!-- https://www.isibang.ac.in/ns/amv#JohnHammersley -->

    <owl:NamedIndividual rdf:about="https://www.isibang.ac.in/ns/amv#JohnHammersley">
        <rdf:type rdf:resource="http://xmlns.com/foaf/0.1/Person"/>
    </owl:NamedIndividual>
    


    <!-- https://www.isibang.ac.in/ns/amv#JohnMauchly -->

    <owl:NamedIndividual rdf:about="https://www.isibang.ac.in/ns/amv#JohnMauchly">
        <rdf:type rdf:resource="http://xmlns.com/foaf/0.1/Person"/>
    </owl:NamedIndividual>
    


    <!-- https://www.isibang.ac.in/ns/amv#K-MeansClusteringAlgorithm -->

    <owl:NamedIndividual rdf:about="https://www.isibang.ac.in/ns/amv#K-MeansClusteringAlgorithm">
        <rdf:type rdf:resource="https://www.isibang.ac.in/ns/amv#Algorithm"/>
        <terms:contributor rdf:resource="https://www.isibang.ac.in/ns/amv#StuartLloyd"/>
        <terms:creator rdf:resource="https://www.isibang.ac.in/ns/amv#EdwardWForgy"/>
        <terms:subject rdf:resource="https://www.isibang.ac.in/ns/amv#Mathematics"/>
        <algorithmAnalysisFunctionType rdf:resource="https://www.isibang.ac.in/ns/amv#ExponentialFunctions"/>
        <loopConstruct rdf:resource="https://www.isibang.ac.in/ns/amv#For"/>
        <terms:created rdf:datatype="http://www.w3.org/2001/XMLSchema#dateTime">1965-01-01T00:00:00</terms:created>
        <terms:description rdf:datatype="http://www.w3.org/2001/XMLSchema#string">K-Means Clustering is an unsupervised learning algorithm, which groups the unlabeled dataset into different clusters. Here K defines the number of pre-defined clusters that need to be created in the process</terms:description>
        <terms:title rdf:datatype="http://www.w3.org/2001/XMLSchema#string">K-Means Clustering</terms:title>
        <Constraint rdf:datatype="http://www.w3.org/2001/XMLSchema#string">The user has to specifyk(the number ofclusters) in the beginning.</Constraint>
        <Constraint rdf:datatype="http://www.w3.org/2001/XMLSchema#string">k-meanscan only handle numerical data.</Constraint>
        <edgeCase rdf:datatype="http://www.w3.org/2001/XMLSchema#string">In the extremecaseforK= N (the number of data points), thenK-meanswill assign each data point to its own separatecluster</edgeCase>
        <flexible rdf:datatype="http://www.w3.org/2001/XMLSchema#boolean">true</flexible>
        <input rdf:datatype="http://www.w3.org/2001/XMLSchema#string">Thealgorithmtakes the unlabeled dataset asinput</input>
    </owl:NamedIndividual>
    


    <!-- https://www.isibang.ac.in/ns/amv#Kd-Trees -->

    <owl:NamedIndividual rdf:about="https://www.isibang.ac.in/ns/amv#Kd-Trees">
        <rdf:type rdf:resource="https://www.isibang.ac.in/ns/amv#DataStructuresProblem"/>
    </owl:NamedIndividual>
    


    <!-- https://www.isibang.ac.in/ns/amv#KenThompson -->

    <owl:NamedIndividual rdf:about="https://www.isibang.ac.in/ns/amv#KenThompson">
        <rdf:type rdf:resource="http://xmlns.com/foaf/0.1/Person"/>
    </owl:NamedIndividual>
    


    <!-- https://www.isibang.ac.in/ns/amv#KnapsackProblemAlgorithm -->

    <owl:NamedIndividual rdf:about="https://www.isibang.ac.in/ns/amv#KnapsackProblemAlgorithm">
        <rdf:type rdf:resource="https://www.isibang.ac.in/ns/amv#Algorithm"/>
        <terms:creator rdf:resource="https://www.isibang.ac.in/ns/amv#TobiasDantzig"/>
        <terms:subject rdf:resource="https://www.isibang.ac.in/ns/amv#Mathematics"/>
        <algorithmAnalysisFunctionType rdf:resource="https://www.isibang.ac.in/ns/amv#ExponentialFunctions"/>
        <algorithmType rdf:resource="https://www.isibang.ac.in/ns/amv#BranchAndBoundAlgorithm"/>
        <algorithmType rdf:resource="https://www.isibang.ac.in/ns/amv#DynamicProgrammingAlgorithm"/>
        <terms:description rdf:datatype="http://www.w3.org/2001/XMLSchema#string">Given a set of items with specific weights and assigned values, the goal is to maximize thevaluein a knapsack while remaining within the weight constraint</terms:description>
        <terms:title rdf:datatype="http://www.w3.org/2001/XMLSchema#string">KnapsackProblemAlgorithm</terms:title>
        <Constraint rdf:datatype="http://www.w3.org/2001/XMLSchema#string">Multiple function calls are expensive. 2) Inefficient when there is lots of branching from one state. 3) Requires large amount of space as the each function state needs to be stored on system stack</Constraint>
        <Readable rdf:datatype="http://www.w3.org/2001/XMLSchema#boolean">true</Readable>
    </owl:NamedIndividual>
    


    <!-- https://www.isibang.ac.in/ns/amv#LinearAlgebra -->

    <owl:NamedIndividual rdf:about="https://www.isibang.ac.in/ns/amv#LinearAlgebra">
        <rdf:type rdf:resource="https://www.isibang.ac.in/ns/amv#Mathematical_Properties"/>
        <rdf:type rdf:resource="https://www.wikidata.org/wiki/Q11862829"/>
    </owl:NamedIndividual>
    


    <!-- https://www.isibang.ac.in/ns/amv#LinearFunctions -->

    <owl:NamedIndividual rdf:about="https://www.isibang.ac.in/ns/amv#LinearFunctions">
        <rdf:type rdf:resource="https://www.isibang.ac.in/ns/amv#AlgorithmAnalysisFunction"/>
    </owl:NamedIndividual>
    


    <!-- https://www.isibang.ac.in/ns/amv#LinearProgramming -->

    <owl:NamedIndividual rdf:about="https://www.isibang.ac.in/ns/amv#LinearProgramming">
        <rdf:type rdf:resource="https://www.isibang.ac.in/ns/amv#NumericalProblem"/>
    </owl:NamedIndividual>
    


    <!-- https://www.isibang.ac.in/ns/amv#LinearSearch -->

    <owl:NamedIndividual rdf:about="https://www.isibang.ac.in/ns/amv#LinearSearch">
        <rdf:type rdf:resource="https://www.isibang.ac.in/ns/amv#CombinatorialProblem"/>
    </owl:NamedIndividual>
    


    <!-- https://www.isibang.ac.in/ns/amv#LinkedList -->

    <owl:NamedIndividual rdf:about="https://www.isibang.ac.in/ns/amv#LinkedList">
        <rdf:type rdf:resource="https://www.isibang.ac.in/ns/amv#DataStructure"/>
    </owl:NamedIndividual>
    


    <!-- https://www.isibang.ac.in/ns/amv#Lisp -->

    <owl:NamedIndividual rdf:about="https://www.isibang.ac.in/ns/amv#Lisp">
        <rdf:type rdf:resource="https://www.wikidata.org/wiki/Q9143#ProgrammingLanguage"/>
    </owl:NamedIndividual>
    


    <!-- https://www.isibang.ac.in/ns/amv#List -->

    <owl:NamedIndividual rdf:about="https://www.isibang.ac.in/ns/amv#List">
        <rdf:type rdf:resource="https://www.isibang.ac.in/ns/amv#DataStructure"/>
    </owl:NamedIndividual>
    


    <!-- https://www.isibang.ac.in/ns/amv#LlewellynThomas -->

    <owl:NamedIndividual rdf:about="https://www.isibang.ac.in/ns/amv#LlewellynThomas">
        <rdf:type rdf:resource="http://xmlns.com/foaf/0.1/Person"/>
    </owl:NamedIndividual>
    


    <!-- https://www.isibang.ac.in/ns/amv#LogarithmicFunction -->

    <owl:NamedIndividual rdf:about="https://www.isibang.ac.in/ns/amv#LogarithmicFunction">
        <rdf:type rdf:resource="https://www.isibang.ac.in/ns/amv#AlgorithmAnalysisFunction"/>
    </owl:NamedIndividual>
    


    <!-- https://www.isibang.ac.in/ns/amv#MS-DOS -->

    <owl:NamedIndividual rdf:about="https://www.isibang.ac.in/ns/amv#MS-DOS">
        <rdf:type rdf:resource="https://schema.org/OperatingSystem"/>
    </owl:NamedIndividual>
    


    <!-- https://www.isibang.ac.in/ns/amv#Mathematics -->

    <owl:NamedIndividual rdf:about="https://www.isibang.ac.in/ns/amv#Mathematics">
        <rdf:type rdf:resource="https://www.wikidata.org/wiki/Q11862829"/>
        <hasBranch rdf:resource="https://www.isibang.ac.in/ns/amv#Graph"/>
        <hasBranch rdf:resource="https://www.isibang.ac.in/ns/amv#LinearAlgebra"/>
    </owl:NamedIndividual>
    


    <!-- https://www.isibang.ac.in/ns/amv#Matlab -->

    <owl:NamedIndividual rdf:about="https://www.isibang.ac.in/ns/amv#Matlab">
        <rdf:type rdf:resource="https://www.wikidata.org/wiki/Q9143#ProgrammingLanguage"/>
    </owl:NamedIndividual>
    


    <!-- https://www.isibang.ac.in/ns/amv#MatrixMultiplication -->

    <owl:NamedIndividual rdf:about="https://www.isibang.ac.in/ns/amv#MatrixMultiplication">
        <rdf:type rdf:resource="https://www.isibang.ac.in/ns/amv#NumericalProblem"/>
    </owl:NamedIndividual>
    


    <!-- https://www.isibang.ac.in/ns/amv#MedianAndSelection -->

    <owl:NamedIndividual rdf:about="https://www.isibang.ac.in/ns/amv#MedianAndSelection">
        <rdf:type rdf:resource="https://www.isibang.ac.in/ns/amv#CombinatorialProblem"/>
    </owl:NamedIndividual>
    


    <!-- https://www.isibang.ac.in/ns/amv#MergeSort -->

    <owl:NamedIndividual rdf:about="https://www.isibang.ac.in/ns/amv#MergeSort">
        <rdf:type rdf:resource="https://www.isibang.ac.in/ns/amv#CombinatorialProblem"/>
    </owl:NamedIndividual>
    


    <!-- https://www.isibang.ac.in/ns/amv#MicrosoftWindows -->

    <owl:NamedIndividual rdf:about="https://www.isibang.ac.in/ns/amv#MicrosoftWindows">
        <rdf:type rdf:resource="https://schema.org/OperatingSystem"/>
    </owl:NamedIndividual>
    


    <!-- https://www.isibang.ac.in/ns/amv#MinimumSpanningTree -->

    <owl:NamedIndividual rdf:about="https://www.isibang.ac.in/ns/amv#MinimumSpanningTree">
        <rdf:type rdf:resource="https://www.isibang.ac.in/ns/amv#PolynomialTimeProblem"/>
    </owl:NamedIndividual>
    


    <!-- https://www.isibang.ac.in/ns/amv#MinimumSpanningTreeAlgorithm -->

    <owl:NamedIndividual rdf:about="https://www.isibang.ac.in/ns/amv#MinimumSpanningTreeAlgorithm">
        <rdf:type rdf:resource="https://www.isibang.ac.in/ns/amv#Algorithm"/>
        <terms:creator rdf:resource="https://www.isibang.ac.in/ns/amv#PerAustrin"/>
        <terms:subject rdf:resource="https://www.isibang.ac.in/ns/amv#Mathematics"/>
        <wdt:p2159 rdf:resource="https://www.isibang.ac.in/ns/amv#MinimumSpanningTree"/>
        <algorithmAnalysisFunctionType rdf:resource="https://www.isibang.ac.in/ns/amv#LogarithmicFunction"/>
        <mathematicalProperty rdf:resource="https://www.isibang.ac.in/ns/amv#GraphTheory"/>
        <terms:description rdf:datatype="http://www.w3.org/2001/XMLSchema#string">A minimum spanning tree (MST) or minimum weight spanning tree is a subset of the edges of a connected, edge-weighted undirected graph that connects all the vertices together, without any cycles and with the minimum possible total edge weight</terms:description>
        <Readable rdf:datatype="http://www.w3.org/2001/XMLSchema#boolean">true</Readable>
        <flexible rdf:datatype="http://www.w3.org/2001/XMLSchema#boolean">true</flexible>
        <input rdf:datatype="http://www.w3.org/2001/XMLSchema#string">Each test case starts with a line with two non-negative integers, 1n200001n20000 and 0m300000m30000, separated by a single space, where nn is the numbers of nodes in the graph and mm is the number of edges</input>
        <numberOfSteps rdf:datatype="http://www.w3.org/2001/XMLSchema#integer">8</numberOfSteps>
    </owl:NamedIndividual>
    


    <!-- https://www.isibang.ac.in/ns/amv#MinkowskiSum -->

    <owl:NamedIndividual rdf:about="https://www.isibang.ac.in/ns/amv#MinkowskiSum">
        <rdf:type rdf:resource="https://www.isibang.ac.in/ns/amv#ComputationalGeometryProblem"/>
    </owl:NamedIndividual>
    


    <!-- https://www.isibang.ac.in/ns/amv#MotionPlanning -->

    <owl:NamedIndividual rdf:about="https://www.isibang.ac.in/ns/amv#MotionPlanning">
        <rdf:type rdf:resource="https://www.isibang.ac.in/ns/amv#ComputationalGeometryProblem"/>
    </owl:NamedIndividual>
    


    <!-- https://www.isibang.ac.in/ns/amv#NSORT -->

    <owl:NamedIndividual rdf:about="https://www.isibang.ac.in/ns/amv#NSORT">
        <rdf:type rdf:resource="https://www.isibang.ac.in/ns/amv#Implementation"/>
        <terms:identifier rdf:datatype="http://www.w3.org/2001/XMLSchema#anyURI">http://www.ordinal.com/</terms:identifier>
        <rdfs:comment xml:lang="en">Nsort is a sort/merge program that can quickly sort large amounts of data, using large numbers of processors and disks in parallel (Source: http://www.ordinal.com/).</rdfs:comment>
    </owl:NamedIndividual>
    


    <!-- https://www.isibang.ac.in/ns/amv#NaturalLanguage -->

    <owl:NamedIndividual rdf:about="https://www.isibang.ac.in/ns/amv#NaturalLanguage">
        <rdf:type rdf:resource="https://www.isibang.ac.in/ns/amv#FormOfExpression"/>
    </owl:NamedIndividual>
    


    <!-- https://www.isibang.ac.in/ns/amv#PerAustrin -->

    <owl:NamedIndividual rdf:about="https://www.isibang.ac.in/ns/amv#PerAustrin">
        <rdf:type rdf:resource="http://xmlns.com/foaf/0.1/Person"/>
    </owl:NamedIndividual>
    


    <!-- https://www.isibang.ac.in/ns/amv#PeterMcIlroy -->

    <owl:NamedIndividual rdf:about="https://www.isibang.ac.in/ns/amv#PeterMcIlroy">
        <rdf:type rdf:resource="http://xmlns.com/foaf/0.1/Person"/>
    </owl:NamedIndividual>
    


    <!-- https://www.isibang.ac.in/ns/amv#PriorityQueues -->

    <owl:NamedIndividual rdf:about="https://www.isibang.ac.in/ns/amv#PriorityQueues">
        <rdf:type rdf:resource="https://www.isibang.ac.in/ns/amv#DataStructuresProblem"/>
    </owl:NamedIndividual>
    


    <!-- https://www.isibang.ac.in/ns/amv#ProgrammingLanguage -->

    <owl:NamedIndividual rdf:about="https://www.isibang.ac.in/ns/amv#ProgrammingLanguage">
        <rdf:type rdf:resource="https://www.isibang.ac.in/ns/amv#FormOfExpression"/>
    </owl:NamedIndividual>
    


    <!-- https://www.isibang.ac.in/ns/amv#Pseudocode -->

    <owl:NamedIndividual rdf:about="https://www.isibang.ac.in/ns/amv#Pseudocode">
        <rdf:type rdf:resource="https://www.isibang.ac.in/ns/amv#FormOfExpression"/>
    </owl:NamedIndividual>
    


    <!-- https://www.isibang.ac.in/ns/amv#Public -->

    <owl:NamedIndividual rdf:about="https://www.isibang.ac.in/ns/amv#Public">
        <rdf:type rdf:resource="http://purl.org/dc/terms/RightsStatement"/>
    </owl:NamedIndividual>
    


    <!-- https://www.isibang.ac.in/ns/amv#Python -->

    <owl:NamedIndividual rdf:about="https://www.isibang.ac.in/ns/amv#Python">
        <rdf:type rdf:resource="https://www.wikidata.org/wiki/Q9143#ProgrammingLanguage"/>
    </owl:NamedIndividual>
    


    <!-- https://www.isibang.ac.in/ns/amv#QuadriticFunction -->

    <owl:NamedIndividual rdf:about="https://www.isibang.ac.in/ns/amv#QuadriticFunction">
        <rdf:type rdf:resource="https://www.isibang.ac.in/ns/amv#AlgorithmAnalysisFunction"/>
    </owl:NamedIndividual>
    


    <!-- https://www.isibang.ac.in/ns/amv#Queue -->

    <owl:NamedIndividual rdf:about="https://www.isibang.ac.in/ns/amv#Queue">
        <rdf:type rdf:resource="https://www.isibang.ac.in/ns/amv#DataStructure"/>
    </owl:NamedIndividual>
    


    <!-- https://www.isibang.ac.in/ns/amv#QuickSort -->

    <owl:NamedIndividual rdf:about="https://www.isibang.ac.in/ns/amv#QuickSort">
        <rdf:type rdf:resource="https://www.isibang.ac.in/ns/amv#CombinatorialProblem"/>
    </owl:NamedIndividual>
    


    <!-- https://www.isibang.ac.in/ns/amv#R -->

    <owl:NamedIndividual rdf:about="https://www.isibang.ac.in/ns/amv#R">
        <rdf:type rdf:resource="https://www.wikidata.org/wiki/Q9143#ProgrammingLanguage"/>
    </owl:NamedIndividual>
    


    <!-- https://www.isibang.ac.in/ns/amv#RandomizedAlgorithm -->

    <owl:NamedIndividual rdf:about="https://www.isibang.ac.in/ns/amv#RandomizedAlgorithm">
        <rdf:type rdf:resource="https://www.isibang.ac.in/ns/amv#AlgorithmicType"/>
    </owl:NamedIndividual>
    


    <!-- https://www.isibang.ac.in/ns/amv#RangeSearch -->

    <owl:NamedIndividual rdf:about="https://www.isibang.ac.in/ns/amv#RangeSearch">
        <rdf:type rdf:resource="https://www.isibang.ac.in/ns/amv#ComputationalGeometryProblem"/>
    </owl:NamedIndividual>
    


    <!-- https://www.isibang.ac.in/ns/amv#RecursiveAlgorithm -->

    <owl:NamedIndividual rdf:about="https://www.isibang.ac.in/ns/amv#RecursiveAlgorithm">
        <rdf:type rdf:resource="https://www.isibang.ac.in/ns/amv#AlgorithmicType"/>
    </owl:NamedIndividual>
    


    <!-- https://www.isibang.ac.in/ns/amv#RedHatLinux -->

    <owl:NamedIndividual rdf:about="https://www.isibang.ac.in/ns/amv#RedHatLinux">
        <rdf:type rdf:resource="https://schema.org/OperatingSystem"/>
    </owl:NamedIndividual>
    


    <!-- https://www.isibang.ac.in/ns/amv#Searching -->

    <owl:NamedIndividual rdf:about="https://www.isibang.ac.in/ns/amv#Searching">
        <rdf:type rdf:resource="https://www.isibang.ac.in/ns/amv#CombinatorialProblem"/>
    </owl:NamedIndividual>
    


    <!-- https://www.isibang.ac.in/ns/amv#SelectionSort -->

    <owl:NamedIndividual rdf:about="https://www.isibang.ac.in/ns/amv#SelectionSort">
        <rdf:type rdf:resource="https://www.isibang.ac.in/ns/amv#CombinatorialProblem"/>
    </owl:NamedIndividual>
    


    <!-- https://www.isibang.ac.in/ns/amv#SelmerMJohnson -->

    <owl:NamedIndividual rdf:about="https://www.isibang.ac.in/ns/amv#SelmerMJohnson">
        <rdf:type rdf:resource="http://xmlns.com/foaf/0.1/Person"/>
    </owl:NamedIndividual>
    


    <!-- https://www.isibang.ac.in/ns/amv#SetCover -->

    <owl:NamedIndividual rdf:about="https://www.isibang.ac.in/ns/amv#SetCover">
        <rdf:type rdf:resource="https://www.isibang.ac.in/ns/amv#SetAndStringProblem"/>
    </owl:NamedIndividual>
    


    <!-- https://www.isibang.ac.in/ns/amv#SetPacking -->

    <owl:NamedIndividual rdf:about="https://www.isibang.ac.in/ns/amv#SetPacking">
        <rdf:type rdf:resource="https://www.isibang.ac.in/ns/amv#SetAndStringProblem"/>
    </owl:NamedIndividual>
    


    <!-- https://www.isibang.ac.in/ns/amv#ShortestPath -->

    <owl:NamedIndividual rdf:about="https://www.isibang.ac.in/ns/amv#ShortestPath">
        <rdf:type rdf:resource="https://www.isibang.ac.in/ns/amv#PolynomialTimeProblem"/>
    </owl:NamedIndividual>
    


    <!-- https://www.isibang.ac.in/ns/amv#SolvingLinearEquations -->

    <owl:NamedIndividual rdf:about="https://www.isibang.ac.in/ns/amv#SolvingLinearEquations">
        <rdf:type rdf:resource="https://www.isibang.ac.in/ns/amv#NumericalProblem"/>
    </owl:NamedIndividual>
    


    <!-- https://www.isibang.ac.in/ns/amv#SortUnix -->

    <owl:NamedIndividual rdf:about="https://www.isibang.ac.in/ns/amv#SortUnix">
        <rdf:type rdf:resource="https://www.isibang.ac.in/ns/amv#Algorithm"/>
        <terms:creator rdf:resource="https://www.isibang.ac.in/ns/amv#KenThompson"/>
        <terms:creator rdf:resource="https://www.isibang.ac.in/ns/amv#At&amp;TBellLaboratories"/>
        <terms:description rdf:datatype="http://www.w3.org/2001/XMLSchema#string">In computing, sort is a standard command line program of Unix and Unix-like operating systems, that prints the lines of its input or concatenation of all files listed in its argument list in sorted order.</terms:description>
    </owl:NamedIndividual>
    


    <!-- https://www.isibang.ac.in/ns/amv#Sorting -->

    <owl:NamedIndividual rdf:about="https://www.isibang.ac.in/ns/amv#Sorting">
        <rdf:type rdf:resource="https://www.isibang.ac.in/ns/amv#CombinatorialProblem"/>
    </owl:NamedIndividual>
    


    <!-- https://www.isibang.ac.in/ns/amv#Statistics -->

    <owl:NamedIndividual rdf:about="https://www.isibang.ac.in/ns/amv#Statistics">
        <rdf:type rdf:resource="https://www.wikidata.org/wiki/Q11862829"/>
    </owl:NamedIndividual>
    


    <!-- https://www.isibang.ac.in/ns/amv#StringMatching -->

    <owl:NamedIndividual rdf:about="https://www.isibang.ac.in/ns/amv#StringMatching">
        <rdf:type rdf:resource="https://www.isibang.ac.in/ns/amv#SetAndStringProblem"/>
    </owl:NamedIndividual>
    


    <!-- https://www.isibang.ac.in/ns/amv#StuartLloyd -->

    <owl:NamedIndividual rdf:about="https://www.isibang.ac.in/ns/amv#StuartLloyd">
        <rdf:type rdf:resource="http://xmlns.com/foaf/0.1/Person"/>
    </owl:NamedIndividual>
    


    <!-- https://www.isibang.ac.in/ns/amv#TextCompression -->

    <owl:NamedIndividual rdf:about="https://www.isibang.ac.in/ns/amv#TextCompression">
        <rdf:type rdf:resource="https://www.isibang.ac.in/ns/amv#SetAndStringProblem"/>
    </owl:NamedIndividual>
    


    <!-- https://www.isibang.ac.in/ns/amv#TheoryOfSets -->

    <owl:NamedIndividual rdf:about="https://www.isibang.ac.in/ns/amv#TheoryOfSets">
        <rdf:type rdf:resource="https://www.isibang.ac.in/ns/amv#Mathematical_Properties"/>
    </owl:NamedIndividual>
    


    <!-- https://www.isibang.ac.in/ns/amv#TheoryOfStatisticsAndProbability -->

    <owl:NamedIndividual rdf:about="https://www.isibang.ac.in/ns/amv#TheoryOfStatisticsAndProbability">
        <rdf:type rdf:resource="https://www.isibang.ac.in/ns/amv#Mathematical_Properties"/>
    </owl:NamedIndividual>
    


    <!-- https://www.isibang.ac.in/ns/amv#TobiasDantzig -->

    <owl:NamedIndividual rdf:about="https://www.isibang.ac.in/ns/amv#TobiasDantzig">
        <rdf:type rdf:resource="http://xmlns.com/foaf/0.1/Person"/>
    </owl:NamedIndividual>
    


    <!-- https://www.isibang.ac.in/ns/amv#TopologicalSorting -->

    <owl:NamedIndividual rdf:about="https://www.isibang.ac.in/ns/amv#TopologicalSorting">
        <rdf:type rdf:resource="https://www.isibang.ac.in/ns/amv#PolynomialTimeProblem"/>
    </owl:NamedIndividual>
    


    <!-- https://www.isibang.ac.in/ns/amv#TowerOfHannoiAlgorithm -->

    <owl:NamedIndividual rdf:about="https://www.isibang.ac.in/ns/amv#TowerOfHannoiAlgorithm">
        <rdf:type rdf:resource="https://www.isibang.ac.in/ns/amv#Algorithm"/>
        <terms:creator rdf:resource="https://www.isibang.ac.in/ns/amv#EdouardLucas"/>
        <terms:subject rdf:resource="https://www.isibang.ac.in/ns/amv#Mathematics"/>
        <algorithmAnalysisFunctionType rdf:resource="https://www.isibang.ac.in/ns/amv#ExponentialFunctions"/>
        <algorithmType rdf:resource="https://www.isibang.ac.in/ns/amv#DivideAndConquerAlgorithm"/>
        <algorithmType rdf:resource="https://www.isibang.ac.in/ns/amv#RecursiveAlgorithm"/>
        <terms:created rdf:datatype="http://www.w3.org/2001/XMLSchema#dateTime">1900-01-01T00:00:00</terms:created>
        <terms:title rdf:datatype="http://www.w3.org/2001/XMLSchema#string">TowerOfHannoi</terms:title>
        <Constraint rdf:datatype="http://www.w3.org/2001/XMLSchema#string">The Tower of Hanoi puzzle is sensitive to prefrontal damage and dysfunction</Constraint>
    </owl:NamedIndividual>
    


    <!-- https://www.isibang.ac.in/ns/amv#TridiagonalMatrixAlgorithm -->

    <owl:NamedIndividual rdf:about="https://www.isibang.ac.in/ns/amv#TridiagonalMatrixAlgorithm">
        <rdf:type rdf:resource="https://www.isibang.ac.in/ns/amv#Algorithm"/>
        <terms:creator rdf:resource="https://www.isibang.ac.in/ns/amv#LlewellynThomas"/>
        <terms:subject rdf:resource="https://www.isibang.ac.in/ns/amv#Mathematics"/>
        <mathematicalProperty rdf:resource="https://www.isibang.ac.in/ns/amv#GaussianElimination"/>
        <terms:description rdf:datatype="http://www.w3.org/2001/XMLSchema#string">It is a simplified form of Gaussian elimination that can be used to solve tridiagonal systems of equations.</terms:description>
        <Optimal rdf:datatype="http://www.w3.org/2001/XMLSchema#boolean">true</Optimal>
        <Readable rdf:datatype="http://www.w3.org/2001/XMLSchema#boolean">true</Readable>
        <flexible rdf:datatype="http://www.w3.org/2001/XMLSchema#boolean">true</flexible>
        <input rdf:datatype="http://www.w3.org/2001/XMLSchema#string">banded matrix</input>
    </owl:NamedIndividual>
    


    <!-- https://www.isibang.ac.in/ns/amv#Unix -->

    <owl:NamedIndividual rdf:about="https://www.isibang.ac.in/ns/amv#Unix">
        <rdf:type rdf:resource="https://schema.org/OperatingSystem"/>
    </owl:NamedIndividual>
    


    <!-- https://www.isibang.ac.in/ns/amv#VaughanPratt -->

    <owl:NamedIndividual rdf:about="https://www.isibang.ac.in/ns/amv#VaughanPratt">
        <rdf:type rdf:resource="http://xmlns.com/foaf/0.1/Person"/>
    </owl:NamedIndividual>
    


    <!-- https://www.isibang.ac.in/ns/amv#VertexColoring -->

    <owl:NamedIndividual rdf:about="https://www.isibang.ac.in/ns/amv#VertexColoring">
        <rdf:type rdf:resource="https://www.isibang.ac.in/ns/amv#HardProblem"/>
    </owl:NamedIndividual>
    


    <!-- https://www.isibang.ac.in/ns/amv#VertexCover -->

    <owl:NamedIndividual rdf:about="https://www.isibang.ac.in/ns/amv#VertexCover">
        <rdf:type rdf:resource="https://www.isibang.ac.in/ns/amv#HardProblem"/>
    </owl:NamedIndividual>
    


    <!-- https://www.isibang.ac.in/ns/amv#VoronoiDiagrams -->

    <owl:NamedIndividual rdf:about="https://www.isibang.ac.in/ns/amv#VoronoiDiagrams">
        <rdf:type rdf:resource="https://www.isibang.ac.in/ns/amv#ComputationalGeometryProblem"/>
    </owl:NamedIndividual>
    


    <!-- https://www.isibang.ac.in/ns/amv#While -->

    <owl:NamedIndividual rdf:about="https://www.isibang.ac.in/ns/amv#While">
        <rdf:type rdf:resource="https://www.isibang.ac.in/ns/amv#LoopConstruct"/>
    </owl:NamedIndividual>
    


    <!-- https://www.isibang.ac.in/ns/amv#WilliamWesleyPeterson -->

    <owl:NamedIndividual rdf:about="https://www.isibang.ac.in/ns/amv#WilliamWesleyPeterson">
        <rdf:type rdf:resource="http://xmlns.com/foaf/0.1/Person"/>
    </owl:NamedIndividual>
    


    <!-- https://www.isibang.ac.in/ns/amv#algorithm000001 -->

    <owl:NamedIndividual rdf:about="https://www.isibang.ac.in/ns/amv#algorithm000001">
        <rdf:type rdf:resource="https://www.isibang.ac.in/ns/amv#Algorithm"/>
    </owl:NamedIndividual>
    


    <!-- https://www.isibang.ac.in/ns/amv#tree -->

    <owl:NamedIndividual rdf:about="https://www.isibang.ac.in/ns/amv#tree">
        <rdf:type rdf:resource="https://www.isibang.ac.in/ns/amv#DataStructure"/>
    </owl:NamedIndividual>
    


    <!-- https://www.isibang.ac.in/ns/amv#tuple -->

    <owl:NamedIndividual rdf:about="https://www.isibang.ac.in/ns/amv#tuple">
        <rdf:type rdf:resource="https://www.isibang.ac.in/ns/amv#DataStructure"/>
    </owl:NamedIndividual>
    


    <!-- https://www.isibang.ac.in/ns/amv#1.0.0 -->

    <owl:NamedIndividual rdf:about="https://www.isibang.ac.in/ns/amv#1.0.0">
        <rdf:type rdf:resource="http://purl.org/dc/elements/1.1/Version"/>
    </owl:NamedIndividual>
    


    <!-- https://www.isibang.ac.in/ns/amv#At&amp;TBellLaboratories -->

    <owl:NamedIndividual rdf:about="https://www.isibang.ac.in/ns/amv#At&amp;TBellLaboratories">
        <rdf:type rdf:resource="http://xmlns.com/foaf/0.1/Organization"/>
    </owl:NamedIndividual>
    


    <!-- https://www.isibang.ac.in/ns/amv#C++ -->

    <owl:NamedIndividual rdf:about="https://www.isibang.ac.in/ns/amv#C++">
        <rdf:type rdf:resource="https://www.wikidata.org/wiki/Q9143#ProgrammingLanguage"/>
    </owl:NamedIndividual>
    


    <!-- https://www.isibang.ac.in/ns/amv#KnuthMorrisPrattAlgorithm -->

    <owl:NamedIndividual rdf:about="https://www.isibang.ac.in/ns/amv#KnuthMorrisPrattAlgorithm">
        <rdf:type rdf:resource="https://www.isibang.ac.in/ns/amv#Algorithm"/>
        <terms:creator rdf:resource="https://www.isibang.ac.in/ns/amv#DonaldKnuth"/>
        <terms:creator rdf:resource="https://www.isibang.ac.in/ns/amv#JamesHMorris"/>
        <terms:creator rdf:resource="https://www.isibang.ac.in/ns/amv#VaughanPratt"/>
        <terms:subject rdf:resource="https://www.isibang.ac.in/ns/amv#ComputerScience"/>
        <algorithmAnalysisFunctionType rdf:resource="https://www.isibang.ac.in/ns/amv#ConstantFunctions"/>
        <algorithmType rdf:resource="https://www.isibang.ac.in/ns/amv#DynamicProgrammingAlgorithm"/>
        <terms:created rdf:datatype="http://www.w3.org/2001/XMLSchema#dateTime">1970-01-01T00:00:00</terms:created>
        <terms:description rdf:datatype="http://www.w3.org/2001/XMLSchema#string">Knuth Morris Pratt(KMP) is analgorithm, which checks the characters from left to right. When a pattern has a sub-pattern appears more than one in the sub-pattern, it uses that property to improve the time complexity, also for in the worst case.</terms:description>
        <terms:title rdf:datatype="http://www.w3.org/2001/XMLSchema#string">Knuth-Morris-Pratt Algorithm</terms:title>
        <Constraint rdf:datatype="http://www.w3.org/2001/XMLSchema#string">It doesnt work well when the size of the alphabets increases. Due to this more and more error occurs.</Constraint>
        <flexible rdf:datatype="http://www.w3.org/2001/XMLSchema#boolean">true</flexible>
        <input rdf:datatype="http://www.w3.org/2001/XMLSchema#string">an array of characters</input>
        <numberOfSteps rdf:datatype="http://www.w3.org/2001/XMLSchema#integer">6</numberOfSteps>
    </owl:NamedIndividual>
    


    <!-- 
    ///////////////////////////////////////////////////////////////////////////////////////
    //
    // General axioms
    //
    ///////////////////////////////////////////////////////////////////////////////////////
     -->

    <rdf:Description>
        <rdf:type rdf:resource="http://www.w3.org/2002/07/owl#AllDifferent"/>
        <owl:distinctMembers rdf:parseType="Collection">
            <rdf:Description rdf:about="https://www.isibang.ac.in/ns/amv#MinimumSpanningTree"/>
            <rdf:Description rdf:about="https://www.isibang.ac.in/ns/amv#MinimumSpanningTreeAlgorithm"/>
        </owl:distinctMembers>
    </rdf:Description>
</rdf:RDF>



<!-- Generated by the OWL API (version 4.5.9.2019-02-01T07:24:44Z) https://github.com/owlcs/owlapi -->

